theories/Core/Semantic/PER/CoreTactics.v
@@ -26,36 +26,36 @@ Ltac destruct_rel_by_assumption in_rel H :=
 Ltac destruct_rel_mod_eval :=
   repeat
     match goal with
-    | H : (forall c c' (equiv_c_c' : {{ Dom c ≈ c' ∈ ?in_rel }}), rel_mod_eval _ _ _ _ _ _ _ _) |- _ =>
+    | H : (forall c c' (equiv_c_c' : {{ Dom c ≈ c' ∈ ?in_rel }}), rel_mod_eval _ _ _ _ _ _ _) |- _ =>
         destruct_rel_by_assumption in_rel H; mark H
-    | H : rel_mod_eval _ _ _ _ _ _ _ _ |- _ =>
+    | H : rel_mod_eval _ _ _ _ _ _ _ |- _ =>
         dependent destruction H
     end;
   unmark_all.
 Ltac destruct_rel_mod_app :=
   repeat
     match goal with
-    | H : (forall c c' (equiv_c_c' : {{ Dom c ≈ c' ∈ ?in_rel }}), rel_mod_app _ _ _ _ _) |- _ =>
+    | H : (forall c c' (equiv_c_c' : {{ Dom c ≈ c' ∈ ?in_rel }}), rel_mod_app _ _ _ _ _ _) |- _ =>
         destruct_rel_by_assumption in_rel H; mark H
-    | H : rel_mod_app _ _ _ _ _ |- _ =>
+    | H : rel_mod_app _ _ _ _ _ _ |- _ =>
         dependent destruction H
     end;
   unmark_all.
-Ltac destruct_rel_typ :=
-  repeat
-    match goal with
-    | H : (forall c c' (equiv_c_c' : {{ Dom c ≈ c' ∈ ?in_rel }}), rel_typ _ _ _ _ _ _ _) |- _ =>
-        destruct_rel_by_assumption in_rel H; mark H
-    | H : rel_typ _ _ _ _ _ _ _ |- _ =>
-        dependent destruction H
-    end;
-  unmark_all.
+(* Ltac destruct_rel_typ := *)
+(*   repeat *)
+(*     match goal with *)
+(*     | H : (forall c c' (equiv_c_c' : {{ Dom c ≈ c' ∈ ?in_rel }}), rel_typ _ _ _ _ _ _ _) |- _ => *)
+(*         destruct_rel_by_assumption in_rel H; mark H *)
+(*     | H : rel_typ _ _ _ _ _ _ _ |- _ => *)
+(*         dependent destruction H *)
+(*     end; *)
+(*   unmark_all. *)
 Ltac destruct_rel_typ_unsorted :=
   repeat
     match goal with
-    | H : (forall c c' (equiv_c_c' : {{ Dom c ≈ c' ∈ ?in_rel }}), rel_typ_unsorted _ _ _ _ _ _) |- _ =>
+    | H : (forall c c' (equiv_c_c' : {{ Dom c ≈ c' ∈ ?in_rel }}), rel_typ_unsorted _ _ _ _ _ _ _) |- _ =>
         destruct_rel_by_assumption in_rel H; mark H
-    | H : rel_typ_unsorted _ _ _ _ _ _ |- _ =>
+    | H : rel_typ_unsorted _ _ _ _ _ _ _ |- _ =>
         dependent destruction H
     end;
   unmark_all.
