theories/Core/Semantic/PER/Lemmas.v
@@ -7,14 +7,14 @@ From McPTS.Core.Syntactic Require Import System.
 From McPTS.Core.Semantic Require Import PER.CoreTactics PER.Definitions.
 Import Domain_Notations.
 
-Add Parametric Morphism {P} R0 `(R0_morphism : Proper _ ((@relation_equivalence (domain P)) ==> (@relation_equivalence (domain P))) R0) A Δ ρ A' Δ' ρ' : (rel_mod_eval R0 A Δ ρ A' Δ' ρ')
+Add Parametric Morphism {P} R0 `(R0_morphism : Proper _ ((@relation_equivalence (domain P)) ==> (@relation_equivalence (domain P))) R0) Δ A ρ A' ρ' : (rel_mod_eval R0 Δ A ρ A' ρ')
     with signature (@relation_equivalence (domain P)) ==> iff as rel_mod_eval_morphism.
 Proof.
   split; intros []; econstructor; try eassumption;
     [> eapply R0_morphism; [symmetry + idtac |]; eassumption ..].
 Qed.
 
-Add Parametric Morphism {P} f a f' a' : (rel_mod_app f a f' a')
+Add Parametric Morphism {P} Δ f a f' a' : (rel_mod_app Δ f a f' a')
     with signature (@relation_equivalence (domain P)) ==> iff as rel_mod_app_morphism.
 Proof.
   intros * HRR'.
@@ -22,25 +22,25 @@ Proof.
     apply HRR'; eassumption.
 Qed.
 
-Lemma per_bot_sym {P} : forall m n : domain_ne P,
-    {{ Dom m ≈ n ∈ per_bot }} ->
-    {{ Dom n ≈ m ∈ per_bot }}.
+Lemma per_bot_sym {P} : forall (Δ : gctx P) m n,
+    {{ Dom m ≈ n ∈ per_bot Δ }} ->
+    {{ Dom n ≈ m ∈ per_bot Δ }}.
 Proof with solve [eauto].
-  intros * H s.
-  pose proof H s.
+  intros * H i.
+  pose proof H i.
   destruct_conjs...
 Qed.
 
 #[export]
 Hint Resolve per_bot_sym : mcpts.
 
-Lemma per_bot_trans {P} : forall m n l : domain_ne P,
-    {{ Dom m ≈ n ∈ per_bot }} ->
-    {{ Dom n ≈ l ∈ per_bot }} ->
-    {{ Dom m ≈ l ∈ per_bot }}.
+Lemma per_bot_trans {P} : forall (Δ : gctx P) m n l,
+    {{ Dom m ≈ n ∈ per_bot Δ }} ->
+    {{ Dom n ≈ l ∈ per_bot Δ }} ->
+    {{ Dom m ≈ l ∈ per_bot Δ }}.
 Proof with solve [eauto].
-  intros * Hmn Hnl s.
-  pose proof (Hmn s, Hnl s).
+  intros * Hmn Hnl i.
+  pose proof (Hmn i, Hnl i).
   destruct_conjs.
   functional_read_rewrite_clear...
 Qed.
@@ -49,15 +49,15 @@ Qed.
 Hint Resolve per_bot_trans : mcpts.
 
 #[export]
-Instance per_bot_PER {P} : PER (@per_bot P).
+Instance per_bot_PER {P} {Δ : gctx P} : PER (per_bot Δ).
 Proof.
   split.
   - eauto using per_bot_sym.
   - eauto using per_bot_trans.
 Qed.
 
-Lemma var_per_bot {P} : forall {n},
-    {{ Dom !n ≈ !n ∈ @per_bot P }}.
+Lemma var_per_bot {P} : forall {Δ : gctx P} {n},
+    {{ Dom !n ≈ !n ∈ per_bot Δ }}.
 Proof.
   intros ? ?. repeat econstructor.
 Qed.
@@ -65,25 +65,34 @@ Qed.
 #[export]
 Hint Resolve var_per_bot : mcpts.
 
-Lemma per_top_sym {P} : forall m n : domain_nf P,
-    {{ Dom m ≈ n ∈ per_top }} ->
-    {{ Dom n ≈ m ∈ per_top }}.
+Lemma gvar_per_bot {P} : forall {Δ : gctx P} {x},
+    {{ Dom `!x ≈ `!x ∈ per_bot Δ }}.
+Proof.
+  intros ? ?. repeat econstructor.
+Qed.
+
+#[export]
+Hint Resolve gvar_per_bot : mcpts.
+
+Lemma per_top_sym {P} : forall {Δ : gctx P} m n,
+    {{ Dom m ≈ n ∈ per_top Δ }} ->
+    {{ Dom n ≈ m ∈ per_top Δ }}.
 Proof with solve [eauto].
-  intros * H s.
-  pose proof H s.
+  intros * H i.
+  pose proof H i.
   destruct_conjs...
 Qed.
 
 #[export]
 Hint Resolve per_top_sym : mcpts.
 
-Lemma per_top_trans {P} : forall m n l : domain_nf P,
-    {{ Dom m ≈ n ∈ per_top }} ->
-    {{ Dom n ≈ l ∈ per_top }} ->
-    {{ Dom m ≈ l ∈ per_top }}.
+Lemma per_top_trans {P} : forall {Δ : gctx P} m n l,
+    {{ Dom m ≈ n ∈ per_top Δ }} ->
+    {{ Dom n ≈ l ∈ per_top Δ }} ->
+    {{ Dom m ≈ l ∈ per_top Δ }}.
 Proof with solve [eauto].
-  intros * Hmn Hnl s.
-  pose proof (Hmn s, Hnl s).
+  intros * Hmn Hnl i.
+  pose proof (Hmn i, Hnl i).
   destruct_conjs.
   functional_read_rewrite_clear...
 Qed.
@@ -92,19 +101,19 @@ Qed.
 Hint Resolve per_top_trans : mcpts.
 
 #[export]
-Instance per_top_PER {P} : PER (@per_top P).
+Instance per_top_PER {P} {Δ : gctx P} : PER (per_top Δ).
 Proof.
   split.
   - eauto using per_top_sym.
   - eauto using per_top_trans.
 Qed.
 
-Lemma per_bot_then_per_top {P} : forall (m : domain_ne P) m' a a' b b' c c',
-    {{ Dom m ≈ m' ∈ per_bot }} ->
-    {{ Dom ⇓ (⇑ a b) ⇑ c m ≈ ⇓ (⇑ a' b') ⇑ c' m' ∈ per_top }}.
+Lemma per_bot_then_per_top {P} : forall {Δ : gctx P} m m' a a' b b' c c',
+    {{ Dom m ≈ m' ∈ per_bot Δ }} ->
+    {{ Dom ⇓ (⇑ a b) ⇑ c m ≈ ⇓ (⇑ a' b') ⇑ c' m' ∈ per_top Δ }}.
 Proof.
-  intros * H s.
-  pose proof H s.
+  intros * H i.
+  pose proof H i.
   destruct_conjs.
   eexists; split; constructor; eassumption.
 Qed.
@@ -112,25 +121,25 @@ Qed.
 #[export]
 Hint Resolve per_bot_then_per_top : mcpts.
 
-Lemma per_top_typ_sym {P} : forall m n : domain P,
-    {{ Dom m ≈ n ∈ per_top_typ }} ->
-    {{ Dom n ≈ m ∈ per_top_typ }}.
+Lemma per_top_typ_sym {P} : forall {Δ : gctx P} m n,
+    {{ Dom m ≈ n ∈ per_top_typ Δ }} ->
+    {{ Dom n ≈ m ∈ per_top_typ Δ }}.
 Proof with solve [eauto].
-  intros * H s.
-  pose proof H s.
+  intros * H i.
+  pose proof H i.
   destruct_conjs...
 Qed.
 
 #[export]
 Hint Resolve per_top_typ_sym : mcpts.
 
-Lemma per_top_typ_trans {P} : forall m n l : domain P,
-    {{ Dom m ≈ n ∈ per_top_typ }} ->
-    {{ Dom n ≈ l ∈ per_top_typ }} ->
-    {{ Dom m ≈ l ∈ per_top_typ }}.
+Lemma per_top_typ_trans {P} : forall {Δ : gctx P} m n l,
+    {{ Dom m ≈ n ∈ per_top_typ Δ }} ->
+    {{ Dom n ≈ l ∈ per_top_typ Δ }} ->
+    {{ Dom m ≈ l ∈ per_top_typ Δ }}.
 Proof with solve [eauto].
-  intros * Hmn Hnl s.
-  pose proof (Hmn s, Hnl s).
+  intros * Hmn Hnl i.
+  pose proof (Hmn i, Hnl i).
   destruct_conjs.
   functional_read_rewrite_clear...
 Qed.
@@ -139,16 +148,17 @@ Qed.
 Hint Resolve per_top_typ_trans : mcpts.
 
 #[export]
-Instance per_top_typ_PER {P} : PER (@per_top_typ P).
+  Instance per_top_typ_PER {P} {Δ : gctx P} : PER (per_top_typ Δ).
 Proof.
   split.
   - eauto using per_top_typ_sym.
   - eauto using per_top_typ_trans.
 Qed.
 
-Lemma per_nat_sym {P} : forall m n : domain P,
-    {{ Dom m ≈ n ∈ per_nat }} ->
-    {{ Dom n ≈ m ∈ per_nat }}.
+
+Lemma per_nat_sym {P} : forall {Δ : gctx P} m n,
+    {{ Dom m ≈ n ∈ per_nat Δ }} ->
+    {{ Dom n ≈ m ∈ per_nat Δ }}.
 Proof with mautosolve.
   induction 1; econstructor...
 Qed.
@@ -156,10 +166,10 @@ Qed.
 #[export]
 Hint Resolve per_nat_sym : mcpts.
 
-Lemma per_nat_trans {P} : forall m n l : domain P,
-    {{ Dom m ≈ n ∈ per_nat }} ->
-    {{ Dom n ≈ l ∈ per_nat }} ->
-    {{ Dom m ≈ l ∈ per_nat }}.
+Lemma per_nat_trans {P} : forall {Δ : gctx P} m n l,
+    {{ Dom m ≈ n ∈ per_nat Δ }} ->
+    {{ Dom n ≈ l ∈ per_nat Δ }} ->
+    {{ Dom m ≈ l ∈ per_nat Δ }}.
 Proof with mautosolve.
   intros * H. gen l.
   induction H; inversion_clear 1; econstructor...
@@ -169,16 +179,17 @@ Qed.
 Hint Resolve per_nat_trans : mcpts.
 
 #[export]
-Instance per_nat_PER {P} : PER (@per_nat P).
+Instance per_nat_PER {P} {Δ : gctx P} : PER (per_nat Δ).
 Proof.
   split.
   - eauto using per_nat_sym.
   - eauto using per_nat_trans.
 Qed.
 
-Lemma per_ne_sym {P} : forall m n : domain P,
-    {{ Dom m ≈ n ∈ per_ne }} ->
-    {{ Dom n ≈ m ∈ per_ne }}.
+
+Lemma per_ne_sym {P} : forall {Δ : gctx P} m n,
+    {{ Dom m ≈ n ∈ per_ne Δ }} ->
+    {{ Dom n ≈ m ∈ per_ne Δ }}.
 Proof with mautosolve.
   intros * [].
   econstructor...
@@ -187,10 +198,10 @@ Qed.
 #[export]
 Hint Resolve per_ne_sym : mcpts.
 
-Lemma per_ne_trans {P} : forall m n l : domain P,
-    {{ Dom m ≈ n ∈ per_ne }} ->
-    {{ Dom n ≈ l ∈ per_ne }} ->
-    {{ Dom m ≈ l ∈ per_ne }}.
+Lemma per_ne_trans {P} : forall {Δ : gctx P} m n l,
+    {{ Dom m ≈ n ∈ per_ne Δ }} ->
+    {{ Dom n ≈ l ∈ per_ne Δ }} ->
+    {{ Dom m ≈ l ∈ per_ne Δ }}.
 Proof with mautosolve.
   intros * [].
   inversion_clear 1.
@@ -201,14 +212,14 @@ Qed.
 Hint Resolve per_ne_trans : mcpts.
 
 #[export]
-Instance per_ne_PER {P} : PER (@per_ne P).
+Instance per_ne_PER {P} {Δ : gctx P} : PER (per_ne Δ).
 Proof.
   split.
   - eauto using per_ne_sym.
   - eauto using per_ne_trans.
 Qed.
 
-Add Parametric Morphism {P} {pred_P : PredicativeSig P} s (per_sort_elem_rec : forall s', pred_rel pred_P s' s -> relation (domain P) -> relation (domain P)) : (per_sort_elem_core pred_P s per_sort_elem_rec)
+Add Parametric Morphism {P} {pred_P : PredicativeSig P} Δ s (per_sort_elem_rec : forall s', pred_rel pred_P s' s -> relation (domain P) -> relation (domain P)) : (per_sort_elem_core pred_P Δ s per_sort_elem_rec)
     with signature (@relation_equivalence (domain P)) ==> eq ==> eq ==> iff as per_sort_elem_core_morphism_iff.
 Proof with mautosolve 3.
   simpl.
@@ -225,14 +236,13 @@ Proof with mautosolve 3.
   all: rewrite HRR'...
 Qed.
 
-Add Parametric Morphism {P} {pred_P : PredicativeSig P} s : (per_sort_elem pred_P s)
+Add Parametric Morphism {P} {pred_P : PredicativeSig P} Δ s : (per_sort_elem pred_P Δ s)
     with signature (@relation_equivalence (domain P)) ==> eq ==> eq ==> iff as per_sort_elem_morphism_iff.
 Proof with mautosolve 3.
   simp per_sort_elem.
   intros R R' HRR'.
 
   split; intros Horig; [gen R' | gen R];
-
     induction Horig;
     eauto;
     try (etransitivity; [symmetry + idtac|]; eassumption);
@@ -243,7 +253,7 @@ Proof with mautosolve 3.
   all: rewrite HRR'...
 Qed.
 
-Add Parametric Morphism {P} {pred_P : PredicativeSig P} s per_sort_rec : (per_sort_elem_core pred_P s per_sort_rec)
+Add Parametric Morphism {P} {pred_P : PredicativeSig P} Δ s per_sort_rec : (per_sort_elem_core pred_P Δ s per_sort_rec)
     with signature (@relation_equivalence (domain P)) ==> (@relation_equivalence (domain P)) as per_sort_elem_core_morphism_relation_equivalence.
 Proof with mautosolve.
   intros * H ? ?.
@@ -252,7 +262,7 @@ Proof with mautosolve.
   reflexivity.
 Qed.
 
-Add Parametric Morphism {P} {pred_P : PredicativeSig P} s : (per_sort_elem pred_P s)
+Add Parametric Morphism {P} {pred_P : PredicativeSig P} Δ s : (per_sort_elem pred_P Δ s)
     with signature (@relation_equivalence (domain P)) ==> (@relation_equivalence (domain P)) as per_sort_elem_morphism_relation_equivalence.
 Proof with mautosolve.
   intros * H ? ?.
@@ -261,7 +271,42 @@ Proof with mautosolve.
   reflexivity.
 Qed.
 
-Add Parametric Morphism {P} {pred_P : PredicativeSig P} s A Δ ρ A' Δ' ρ' : (rel_typ pred_P s A Δ ρ A' Δ' ρ')
+(* Add Parametric Morphism {P} {pred_P : PredicativeSig P} s Δ A ρ A' ρ' : (rel_typ pred_P s Δ A ρ A' ρ') *)
+(*     with signature (@relation_equivalence (domain P)) ==> iff as rel_typ_morphism. *)
+(* Proof. *)
+(*   intros * HRR'. *)
+(*   split; intros []; econstructor; try eassumption; *)
+(*     [setoid_rewrite <- HRR' | setoid_rewrite HRR']; eassumption. *)
+(* Qed. *)
+
+
+Add Parametric Morphism {P} {pred_P : PredicativeSig P} Δ : (per_typ_elem pred_P Δ)
+    with signature (@relation_equivalence (domain P)) ==> eq ==> eq ==> iff as per_typ_elem_morphism_iff.
+Proof with mautosolve 3.
+  simp per_sort_elem.
+  intros R R' HRR'.
+
+  split; intros Horig; [gen R' | gen R];
+    induction Horig;
+    eauto;
+    try (etransitivity; [symmetry + idtac|]; eassumption);
+    intros;
+    destruct_rel_mod_eval;
+    econstructor; mauto 3.
+  1-2: rewrite <- HRR'...
+  all: rewrite HRR'...
+Qed.
+
+Add Parametric Morphism {P} {pred_P : PredicativeSig P} Δ : (per_typ_elem pred_P Δ)
+    with signature (@relation_equivalence (domain P)) ==> (@relation_equivalence (domain P)) as per_sort_typ_morphism_relation_equivalence.
+Proof with mautosolve.
+  intros * H ? ?.
+  simpl.
+  rewrite H.
+  reflexivity.
+Qed.
+
+Add Parametric Morphism {P} {pred_P : PredicativeSig P} Δ A ρ A' ρ' : (rel_typ_unsorted pred_P Δ A ρ A' ρ')
     with signature (@relation_equivalence (domain P)) ==> iff as rel_typ_morphism.
 Proof.
   intros * HRR'.
@@ -269,14 +314,15 @@ Proof.
     [setoid_rewrite <- HRR' | setoid_rewrite HRR']; eassumption.
 Qed.
 
-Lemma domain_app_per {P} : forall (f : domain_ne P) f' a a',
-  {{ Dom f ≈ f' ∈ per_bot }} ->
-  {{ Dom a ≈ a' ∈ per_top }} ->
-  {{ Dom f a ≈ f' a' ∈ per_bot }}.
+
+Lemma domain_app_per {P} : forall {Δ : gctx P}f f' a a',
+  {{ Dom f ≈ f' ∈ per_bot Δ }} ->
+  {{ Dom a ≈ a' ∈ per_top Δ }} ->
+  {{ Dom f a ≈ f' a' ∈ per_bot Δ }}.
 Proof.
-  intros. intros s.
-  destruct (H s) as [? []].
-  destruct (H0 s) as [? []].
+  intros. intros i.
+  destruct (H i) as [? []].
+  destruct (H0 i) as [? []].
   mauto.
 Qed.
 
@@ -311,23 +357,23 @@ Ltac apply_relation_equivalence :=
   rewrite_relation_equivalence_left;
   clear_relation_equivalence.
 
-Lemma per_sort_elem_pi_arg_helper {P} {pred_P : PredicativeSig P} : forall {s_in s_out s_pi s_elem a a' in_rel},
+Lemma per_sort_elem_pi_arg_helper {P} {pred_P : PredicativeSig P} : forall {Δ s_in s_out s_pi s_elem a a' in_rel},
     Ru_pi P s_in s_out s_pi ->
     st_subtyp s_pi s_elem ->
-    (s_in = s_elem -> {{ DF a ≈ a' ∈ per_sort_elem pred_P s_elem ↘ in_rel }}) /\ (pred_rel pred_P s_in s_elem -> {{ DF a ≈ a' ∈ per_sort_elem pred_P s_in ↘ in_rel }}) <-> {{ DF a ≈ a' ∈ per_sort_elem pred_P s_in ↘ in_rel }}.
+    (s_in = s_elem -> {{ DF a ≈ a' ∈ per_sort_elem pred_P Δ s_elem ↘ in_rel }}) /\ (pred_rel pred_P s_in s_elem -> {{ DF a ≈ a' ∈ per_sort_elem pred_P Δ s_in ↘ in_rel }}) <-> {{ DF a ≈ a' ∈ per_sort_elem pred_P Δ s_in ↘ in_rel }}.
 Proof.
   intros * r sub.
   split; [intros [Heq Hlt] | split; intros; subst; eauto].
   destruct (ord_ru_pi_sub pred_P r sub) as [[|] _]; subst; eauto.
 Qed.
 
-Lemma per_sort_elem_pi_ret_helper {P} {pred_P : PredicativeSig P} : forall {s_in s_out s_pi s_elem Δ ρ B Δ' ρ' B' in_rel} (out_rel : forall {n n'}, {{ Dom n ≈ n' ∈ in_rel }} -> relation (domain P)),
+Lemma per_sort_elem_pi_ret_helper {P} {pred_P : PredicativeSig P} : forall {Δ s_in s_out s_pi s_elem ρ B ρ' B' in_rel} (out_rel : forall {n n'}, {{ Dom n ≈ n' ∈ in_rel }} -> relation (domain P)),
     Ru_pi P s_in s_out s_pi ->
     st_subtyp s_pi s_elem ->
     (forall n n' (equiv_n_n' : {{ Dom n ≈ n' ∈ in_rel }}),
-        rel_mod_eval (fun R b b' => (s_out = s_elem -> {{ DF b ≈ b' ∈ per_sort_elem pred_P s_elem ↘ R }}) /\ (pred_rel pred_P s_out s_elem -> {{ DF b ≈ b' ∈ per_sort_elem pred_P s_out ↘ R }})) B Δ d{{{ ρ ↦ n }}} B' Δ' d{{{ ρ' ↦ n' }}} (out_rel equiv_n_n')) <->
+        rel_mod_eval (fun R b b' => (s_out = s_elem -> {{ DF b ≈ b' ∈ per_sort_elem pred_P Δ s_elem ↘ R }}) /\ (pred_rel pred_P s_out s_elem -> {{ DF b ≈ b' ∈ per_sort_elem pred_P Δ s_out ↘ R }})) Δ B d{{{ ρ ↦ n }}} B' d{{{ ρ' ↦ n' }}} (out_rel equiv_n_n')) <->
       (forall n n' (equiv_n_n' : {{ Dom n ≈ n' ∈ in_rel }}),
-          rel_mod_eval (per_sort_elem pred_P s_out) B Δ d{{{ ρ ↦ n }}} B' Δ' d{{{ ρ' ↦ n' }}} (out_rel equiv_n_n')).
+          rel_mod_eval (per_sort_elem pred_P Δ s_out) Δ B d{{{ ρ ↦ n }}} B' d{{{ ρ' ↦ n' }}} (out_rel equiv_n_n')).
 Proof.
   intros * r sub.
   split;
@@ -337,21 +383,21 @@ Proof.
   - split; intros; subst; eauto.
 Qed.
 
-Lemma per_sort_elem_pi_left_inversion {P} {pred_P : PredicativeSig P} : forall {s_in s_out s s'} {r : Ru_pi P s_in s_out s} {a Δ ρ B c' elem_rel},
-    {{ DF Π r a (Δ ; ρ) B ≈ c' ∈ per_sort_elem pred_P s' ↘ elem_rel }} ->
-    exists a' Δ' ρ' B' in_rel (out_rel : forall {n n'} (equiv_n_n' : {{ Dom n ≈ n' ∈ in_rel }}), relation (domain P)),
+Lemma per_sort_elem_pi_left_inversion {P} {pred_P : PredicativeSig P} : forall {Δ s_in s_out s s'} {r : Ru_pi P s_in s_out s} {a ρ B c' elem_rel},
+    {{ DF Π r a ρ B ≈ c' ∈ per_sort_elem pred_P Δ s' ↘ elem_rel }} ->
+    exists a' ρ' B' in_rel (out_rel : forall {n n'} (equiv_n_n' : {{ Dom n ≈ n' ∈ in_rel }}), relation (domain P)),
       st_subtyp s s' /\
-      c' = d{{{ Π r a' (Δ' ; ρ') B' }}} /\
-        {{ DF a ≈ a' ∈ per_sort_elem pred_P s_in ↘ in_rel }} /\
+      c' = d{{{ Π r a' ρ' B' }}} /\
+        {{ DF a ≈ a' ∈ per_sort_elem pred_P Δ s_in ↘ in_rel }} /\
         (forall n n' (equiv_n_n' : {{ Dom n ≈ n' ∈ in_rel }}),
-            rel_mod_eval (per_sort_elem pred_P s_out) B Δ d{{{ ρ ↦ n }}} B' Δ' d{{{ ρ' ↦ n' }}} (out_rel equiv_n_n')) /\
-        (elem_rel <~> fun f f' => forall n n' (equiv_n_n' : {{ Dom n ≈ n' ∈ in_rel }}), rel_mod_app f n f' n' (out_rel equiv_n_n')).
+            rel_mod_eval (per_sort_elem pred_P Δ s_out) Δ B d{{{ ρ ↦ n }}} B' d{{{ ρ' ↦ n' }}} (out_rel equiv_n_n')) /\
+        (elem_rel <~> fun f f' => forall n n' (equiv_n_n' : {{ Dom n ≈ n' ∈ in_rel }}), rel_mod_app Δ f n f' n' (out_rel equiv_n_n')).
 Proof.
   intros * H.
   basic_invert_per_sort_elem H.
   erewrite (per_sort_elem_pi_arg_helper r sub) in equiv_a_a'.
   erewrite (per_sort_elem_pi_ret_helper _ r sub) in H0.
-  eexists a', Δ', ρ', B', in_rel, out_rel; eauto.
+  eexists a', ρ', B', in_rel, out_rel; eauto.
 Qed.
 
 #[local]
@@ -359,21 +405,21 @@ Ltac invert_per_sort_elem' H :=
   (unshelve eapply per_sort_elem_pi_left_inversion in H; shelve_unifiable; deex_in H; destruct H as [-> [-> [? []]]])
   + basic_invert_per_sort_elem H.
 
-Lemma per_sort_elem_right_irrel {P} {pred_P : PredicativeSig P} : forall s s' R a b R' b',
-    {{ DF a ≈ b ∈ per_sort_elem pred_P s ↘ R }} ->
-    {{ DF a ≈ b' ∈ per_sort_elem pred_P s' ↘ R' }} ->
+Lemma per_sort_elem_right_irrel {P} {pred_P : PredicativeSig P} : forall Δ s s' R a b R' b',
+    {{ DF a ≈ b ∈ per_sort_elem pred_P Δ s ↘ R }} ->
+    {{ DF a ≈ b' ∈ per_sort_elem pred_P Δ s' ↘ R' }} ->
     (R <~> R').
 Proof with (destruct_rel_mod_eval; destruct_rel_mod_app; functional_eval_rewrite_clear; econstructor; intuition).
   simpl.
   intros * Horig.
   remember a as a' in |- *.
   gen s' a' b' R'.
-
   induction Horig using @per_sort_elem_ind; mauto; intros * ? ? Hright; subst;
     invert_per_sort_elem' Hright;
     apply_relation_equivalence;
     try reflexivity.
-  assert (per_sort_elem pred_P s_in in_rel0 a a'0).
+
+  assert (per_sort_elem pred_P Δ s_in in_rel0 a a'0).
   {
     destruct equiv_a_a' as [equiv_a_a'_eq equiv_a_a'_rel].
     pose proof ord_ru_pi_sub pred_P r sub0 as [].
@@ -382,24 +428,23 @@ Proof with (destruct_rel_mod_eval; destruct_rel_mod_app; functional_eval_rewrite
   assert (in_rel <~> in_rel0) by mauto 3.
   split; intros.
   - rename equiv_n_n' into equiv0_n_n'.
-    specialize (H4 n n' equiv0_n_n').
-    inversion_clear H4.
-    assert (per_sort_elem pred_P s_out (out_rel0 n n' equiv0_n_n') a0 a'1).
+    assert (in_rel n n') as equiv_n_n' by intuition.
+    destruct_rel_mod_eval.
+    simplify_evals.
+    
+    (* specialize (H4 n n' equiv0_n_n'). *)
+    (* inversion_clear H4. *)
+    assert (per_sort_elem pred_P Δ s_out (out_rel0 n n' equiv0_n_n') a0 a'1).
     {
-      destruct H9.
-      pose proof ord_ru_pi_sub pred_P r sub0 as [].
-      destruct H11; subst; mauto 3.
+      pose proof ord_ru_pi_sub pred_P r sub0 as [? []]; subst; mauto 3.
     }
-    assert (equiv_n_n' : in_rel n n') by firstorder...
+    idtac...
     
   - assert (equiv0_n_n' : in_rel0 n n') by firstorder.
-    specialize (H4 n n' equiv0_n_n').
-    inversion_clear H4.
-    assert (per_sort_elem pred_P s_out (out_rel0 n n' equiv0_n_n') a0 a'1).
+    destruct_rel_mod_eval.
+    assert (per_sort_elem pred_P Δ s_out (out_rel0 n n' equiv0_n_n') a0 a'1).
     {
-      destruct H9.
-      pose proof ord_ru_pi_sub pred_P r sub0 as [].
-      destruct H11; subst; mauto 3.
+      pose proof ord_ru_pi_sub pred_P r sub0 as [? []]; subst; mauto 3.
     }
     idtac...
 Qed.
@@ -407,8 +452,8 @@ Qed.
 #[local]
 Ltac per_sort_elem_right_irrel_assert1 :=
   match goal with
-  | H1 : {{ DF ^?a ≈ ^?b ∈ per_sort_elem ?pred_P ?s ↘ ?R1 }},
-      H2 : {{ DF ^?a ≈ ^?b' ∈ per_sort_elem ?pred_P ?s ↘ ?R2 }} |- _ =>
+  | H1 : {{ DF ^?a ≈ ^?b ∈ per_sort_elem ?pred_P ?Δ ?s ↘ ?R1 }},
+      H2 : {{ DF ^?a ≈ ^?b' ∈ per_sort_elem ?pred_P ?Δ ?s ↘ ?R2 }} |- _ =>
       assert_fails (unify R1 R2);
       match goal with
       | H : R1 <~> R2 |- _ => fail 1
@@ -419,12 +464,12 @@ Ltac per_sort_elem_right_irrel_assert1 :=
 #[local]
 Ltac per_sort_elem_right_irrel_assert := repeat per_sort_elem_right_irrel_assert1.
 
-Lemma per_sort_elem_pi_econstructor {P} {pred_P : PredicativeSig P} : forall {s_in s_out s_pi s a Δ ρ B a' Δ' ρ' B'} (r : Ru_pi P s_in s_out s_pi) (sub : st_subtyp s_pi s) {in_rel} (out_rel : forall {n n'}, {{ Dom n ≈ n' ∈ in_rel }} -> relation (domain P)) {elem_rel} (equiv_a_a' : {{ DF a ≈ a' ∈ per_sort_elem pred_P s_in ↘ in_rel }}),
+Lemma per_sort_elem_pi_econstructor {P} {pred_P : PredicativeSig P} : forall {Δ s_in s_out s_pi s a ρ B a' ρ' B'} (r : Ru_pi P s_in s_out s_pi) (sub : st_subtyp s_pi s) {in_rel} (out_rel : forall {n n'}, {{ Dom n ≈ n' ∈ in_rel }} -> relation (domain P)) {elem_rel} (equiv_a_a' : {{ DF a ≈ a' ∈ per_sort_elem pred_P Δ s_in ↘ in_rel }}),
     PER in_rel ->
     (forall {n n'} (equiv_n_n' : {{ Dom n ≈ n' ∈ in_rel }}),
-        rel_mod_eval (per_sort_elem pred_P s_out) B Δ d{{{ ρ ↦ n }}} B' Δ' d{{{ ρ' ↦ n' }}} (out_rel equiv_n_n')) ->
-    (elem_rel <~> fun f f' => forall n n' (equiv_n_n' : {{ Dom n ≈ n' ∈ in_rel }}), rel_mod_app f n f' n' (out_rel equiv_n_n')) ->
-    {{ DF Π r a (Δ ; ρ) B ≈ Π r a' (Δ' ; ρ') B' ∈ per_sort_elem pred_P s ↘ elem_rel }}.
+        rel_mod_eval (per_sort_elem pred_P Δ s_out) Δ B d{{{ ρ ↦ n }}} B' d{{{ ρ' ↦ n' }}} (out_rel equiv_n_n')) ->
+    (elem_rel <~> fun f f' => forall n n' (equiv_n_n' : {{ Dom n ≈ n' ∈ in_rel }}), rel_mod_app Δ f n f' n' (out_rel equiv_n_n')) ->
+    {{ DF Π r a ρ B ≈ Π r a' ρ' B' ∈ per_sort_elem pred_P Δ s ↘ elem_rel }}.
 Proof.
   intros.
   rewrite <- (per_sort_elem_pi_arg_helper r sub) in equiv_a_a'.
@@ -436,9 +481,9 @@ Qed.
 Ltac per_sort_elem_econstructor' :=
   (repeat intro; hnf; eapply per_sort_elem_pi_econstructor) + basic_per_sort_elem_econstructor.
 
-Lemma per_sort_elem_sym {P} {pred_P : PredicativeSig P} : forall {s R a b},
-    {{ DF a ≈ b ∈ per_sort_elem pred_P s ↘ R }} ->
-    {{ DF b ≈ a ∈ per_sort_elem pred_P s ↘ R }} /\
+Lemma per_sort_elem_sym {P} {pred_P : PredicativeSig P} : forall {Δ s R a b},
+    {{ DF a ≈ b ∈ per_sort_elem pred_P Δ s ↘ R }} ->
+    {{ DF b ≈ a ∈ per_sort_elem pred_P Δ s ↘ R }} /\
       (forall m m',
           {{ Dom m ≈ m' ∈ R }} ->
           {{ Dom m' ≈ m ∈ R }}).
@@ -479,24 +524,24 @@ Proof with mautosolve.
   - split; [per_sort_elem_econstructor' | apply_relation_equivalence]; mauto 3.
 Qed.
 
-Corollary per_sort_sym {P} {pred_P : PredicativeSig P} : forall s R a b,
-    {{ DF a ≈ b ∈ per_sort_elem pred_P s ↘ R }} ->
-    {{ DF b ≈ a ∈ per_sort_elem pred_P s ↘ R }}.
+Corollary per_sort_sym {P} {pred_P : PredicativeSig P} : forall Δ s R a b,
+    {{ DF a ≈ b ∈ per_sort_elem pred_P Δ s ↘ R }} ->
+    {{ DF b ≈ a ∈ per_sort_elem pred_P Δ s ↘ R }}.
 Proof.
   intros * ?%per_sort_elem_sym.
   firstorder.
 Qed.
 
-Corollary per_sort_sym' {P} {pred_P : PredicativeSig P} : forall s a b,
-    {{ Dom a ≈ b ∈ per_sort pred_P s }} ->
-    {{ Dom b ≈ a ∈ per_sort pred_P s }}.
+Corollary per_sort_sym' {P} {pred_P : PredicativeSig P} : forall Δ s a b,
+    {{ Dom a ≈ b ∈ per_sort pred_P Δ s }} ->
+    {{ Dom b ≈ a ∈ per_sort pred_P Δ s }}.
 Proof.
   intros * [? ?%per_sort_elem_sym].
   firstorder.
 Qed.
 
-Corollary per_elem_sym {P} {pred_P : PredicativeSig P} : forall s R a b m m',
-    {{ DF a ≈ b ∈ per_sort_elem pred_P s ↘ R }} ->
+Corollary per_elem_sym {P} {pred_P : PredicativeSig P} : forall Δ s R a b m m',
+    {{ DF a ≈ b ∈ per_sort_elem pred_P Δ s ↘ R }} ->
     {{ Dom m ≈ m' ∈ R }} ->
     {{ Dom m' ≈ m ∈ R }}.
 Proof.
@@ -504,18 +549,18 @@ Proof.
   firstorder.
 Qed.
 
-Corollary per_sort_elem_left_irrel {P} {pred_P : PredicativeSig P} : forall s s' R a b R' a',
-    {{ DF a ≈ b ∈ per_sort_elem pred_P s ↘ R }} ->
-    {{ DF a' ≈ b ∈ per_sort_elem pred_P s' ↘ R' }} ->
+Corollary per_sort_elem_left_irrel {P} {pred_P : PredicativeSig P} : forall Δ s s' R a b R' a',
+    {{ DF a ≈ b ∈ per_sort_elem pred_P Δ s ↘ R }} ->
+    {{ DF a' ≈ b ∈ per_sort_elem pred_P Δ s' ↘ R' }} ->
     (R <~> R').
 Proof.
   intros * ?%per_sort_sym ?%per_sort_sym.
   eauto using per_sort_elem_right_irrel.
 Qed.
 
-Corollary per_sort_elem_cross_irrel {P} {pred_P : PredicativeSig P} : forall s s' R a b R' b',
-    {{ DF a ≈ b ∈ per_sort_elem pred_P s ↘ R }} ->
-    {{ DF b' ≈ a ∈ per_sort_elem pred_P s' ↘ R' }} ->
+Corollary per_sort_elem_cross_irrel {P} {pred_P : PredicativeSig P} : forall Δ s s' R a b R' b',
+    {{ DF a ≈ b ∈ per_sort_elem pred_P Δ s ↘ R }} ->
+    {{ DF b' ≈ a ∈ per_sort_elem pred_P Δ s' ↘ R' }} ->
     (R <~> R').
 Proof.
   intros * ? ?%per_sort_sym.
@@ -525,24 +570,24 @@ Qed.
 Ltac do_per_sort_elem_irrel_assert1 :=
   let tactic_error o1 o2 := fail 2 "per_sort_elem_irrel biconditional between" o1 "and" o2 "cannot be solved" in
   match goal with
-  | H1 : {{ DF ^?a ≈ ^_ ∈ per_sort_elem ?pred_P ?s ↘ ?R1 }},
-      H2 : {{ DF ^?a ≈ ^_ ∈ per_sort_elem ?pred_P ?s' ↘ ?R2 }} |- _ =>
+  | H1 : {{ DF ^?a ≈ ^_ ∈ per_sort_elem ?pred_P ?Δ ?s ↘ ?R1 }},
+      H2 : {{ DF ^?a ≈ ^_ ∈ per_sort_elem ?pred_P ?Δ ?s' ↘ ?R2 }} |- _ =>
       assert_fails (unify R1 R2);
       match goal with
       | H : R1 <~> R2 |- _ => fail 1
       | H : R2 <~> R1 |- _ => fail 1
       | _ => assert (R1 <~> R2) by (eapply per_sort_elem_right_irrel; [apply H1 | apply H2]) || tactic_error R1 R2
       end
-  | H1 : {{ DF ^_ ≈ ^?b ∈ per_sort_elem ?pred_P ?s ↘ ?R1 }},
-      H2 : {{ DF ^_ ≈ ^?b ∈ per_sort_elem ?pred_P ?s' ↘ ?R2 }} |- _ =>
+  | H1 : {{ DF ^_ ≈ ^?b ∈ per_sort_elem ?pred_P ?Δ ?s ↘ ?R1 }},
+      H2 : {{ DF ^_ ≈ ^?b ∈ per_sort_elem ?pred_P ?Δ ?s' ↘ ?R2 }} |- _ =>
       assert_fails (unify R1 R2);
       match goal with
       | H : R1 <~> R2 |- _ => fail 1
       | H : R2 <~> R1 |- _ => fail 1
       | _ => assert (R1 <~> R2) by (eapply per_sort_elem_left_irrel; [apply H1 | apply H2]) || tactic_error R1 R2
       end
-  | H1 : {{ DF ^?a ≈ ^_ ∈ per_sort_elem ?pred_P ?s ↘ ?R1 }},
-      H2 : {{ DF ^_ ≈ ^?a ∈ per_sort_elem ?pred_P ?s' ↘ ?R2 }} |- _ =>
+  | H1 : {{ DF ^?a ≈ ^_ ∈ per_sort_elem ?pred_P ?Δ ?s ↘ ?R1 }},
+      H2 : {{ DF ^_ ≈ ^?a ∈ per_sort_elem ?pred_P ?Δ ?s' ↘ ?R2 }} |- _ =>
       (** Order matters less here as H1 and H2 cannot be exchanged *)
       assert_fails (unify R1 R2);
       match goal with
@@ -561,11 +606,11 @@ Ltac handle_per_sort_elem_irrel :=
   apply_relation_equivalence;
   clear_dups.
 
-Lemma per_sort_elem_trans {P : PtsSig} {pred_P : PredicativeSig P} : forall s R a1 a2,
-    {{ DF a1 ≈ a2 ∈ per_sort_elem pred_P s ↘ R }} ->
+Lemma per_sort_elem_trans {P : PtsSig} {pred_P : PredicativeSig P} : forall Δ s R a1 a2,
+    {{ DF a1 ≈ a2 ∈ per_sort_elem pred_P Δ s ↘ R }} ->
     (forall s' a3,
-        {{ DF a2 ≈ a3 ∈ per_sort_elem pred_P s' ↘ R }} ->
-        {{ DF a1 ≈ a3 ∈ per_sort_elem pred_P s ↘ R }}) /\
+        {{ DF a2 ≈ a3 ∈ per_sort_elem pred_P Δ s' ↘ R }} ->
+        {{ DF a1 ≈ a3 ∈ per_sort_elem pred_P Δ s ↘ R }}) /\
       (forall m1 m2 m3,
           R m1 m2 ->
           R m2 m3 ->
@@ -585,7 +630,7 @@ Proof with (per_sort_elem_econstructor'; mautosolve 4).
   - (* pi case *)
     destruct_conjs.
     pose proof (ord_ru_pi_sub pred_P r sub0) as [ord_dom ord_im].
-    assert (per_sort_elem pred_P s_in in_rel0 a' a'0) by (destruct ord_dom; subst; mauto 2).
+    assert (per_sort_elem pred_P Δ s_in in_rel0 a' a'0) by (destruct ord_dom; subst; mauto 2).
     per_sort_elem_econstructor'; eauto.
     + handle_per_sort_elem_irrel.
       intuition.
@@ -593,7 +638,7 @@ Proof with (per_sort_elem_econstructor'; mautosolve 4).
       pose proof (H4 n n' equiv_n_n').
       inversion_clear H11.
       destruct_conjs.
-      assert (per_sort_elem pred_P s_out (out_rel0 n n' equiv_n_n') a0 a'1) by (destruct ord_im; subst; mauto 2).
+      assert (per_sort_elem pred_P Δ s_out (out_rel0 n n' equiv_n_n') a0 a'1) by (destruct ord_im; subst; mauto 2).
       handle_per_sort_elem_irrel.
       assert (in_rel n n') by firstorder.
       assert (in_rel n n) by intuition.
@@ -620,27 +665,27 @@ Proof with (per_sort_elem_econstructor'; mautosolve 4).
     idtac...
 Qed.
 
-Corollary per_sort_trans {P : PtsSig} {pred_P : PredicativeSig P} : forall s s' R a1 a2 a3,
-    per_sort_elem pred_P s R a1 a2 ->
-    per_sort_elem pred_P s' R a2 a3 ->
-    per_sort_elem pred_P s R a1 a3.
+Corollary per_sort_trans {P : PtsSig} {pred_P : PredicativeSig P} : forall Δ s s' R a1 a2 a3,
+    per_sort_elem pred_P Δ s R a1 a2 ->
+    per_sort_elem pred_P Δ s' R a2 a3 ->
+    per_sort_elem pred_P Δ s R a1 a3.
 Proof.
   intros * ?%per_sort_elem_trans.
   firstorder.
 Qed.
 
-Corollary per_sort_trans' {P : PtsSig} {pred_P : PredicativeSig P} : forall s s' a1 a2 a3,
-    {{ Dom a1 ≈ a2 ∈ per_sort pred_P s }} ->
-    {{ Dom a2 ≈ a3 ∈ per_sort pred_P s' }} ->
-    {{ Dom a1 ≈ a3 ∈ per_sort pred_P s }}.
+Corollary per_sort_trans' {P : PtsSig} {pred_P : PredicativeSig P} : forall Δ s s' a1 a2 a3,
+    {{ Dom a1 ≈ a2 ∈ per_sort pred_P Δ s }} ->
+    {{ Dom a2 ≈ a3 ∈ per_sort pred_P Δ s' }} ->
+    {{ Dom a1 ≈ a3 ∈ per_sort pred_P Δ s }}.
 Proof.
   intros * [? ?] [? ?].
   handle_per_sort_elem_irrel.
   firstorder mauto using per_sort_trans.
 Qed.
 
-Corollary per_elem_trans {P : PtsSig} {pred_P : PredicativeSig P} : forall s R a1 a2 m1 m2 m3,
-    per_sort_elem pred_P s R a1 a2 ->
+Corollary per_elem_trans {P : PtsSig} {pred_P : PredicativeSig P} : forall Δ s R a1 a2 m1 m2 m3,
+    per_sort_elem pred_P Δ s R a1 a2 ->
     R m1 m2 ->
     R m2 m3 ->
     R m1 m3.
@@ -650,7 +695,7 @@ Proof.
 Qed.
 
 #[export]
-Instance per_sort_PER {P : PtsSig} {pred_P : PredicativeSig P} {s R} : PER (per_sort_elem pred_P s R).
+Instance per_sort_PER {P : PtsSig} {pred_P : PredicativeSig P} {Δ s R} : PER (per_sort_elem pred_P Δ s R).
 Proof.
   split.
   - auto using per_sort_sym.
@@ -658,7 +703,7 @@ Proof.
 Qed.
 
 #[export]
-Instance per_sort_PER' {P : PtsSig} {pred_P : PredicativeSig P} {s} : PER (per_sort pred_P s).
+Instance per_sort_PER' {P : PtsSig} {pred_P : PredicativeSig P} {Δ s} : PER (per_sort pred_P Δ s).
 Proof.
   split.
   - auto using per_sort_sym'.
@@ -666,343 +711,18 @@ Proof.
 Qed.
 
 #[export]
-Instance per_elem_PER {P : PtsSig} {pred_P : PredicativeSig P} {s R a b} (H : per_sort_elem pred_P s R a b) : PER R.
+Instance per_elem_PER {P : PtsSig} {pred_P : PredicativeSig P} {Δ s R a b} (H : per_sort_elem pred_P Δ s R a b) : PER R.
 Proof.
   split.
-  - pose proof (fun m m' => per_elem_sym _ _ _ _ m m' H). eauto.
-  - pose proof (fun m0 m1 m2 => per_elem_trans _ _ _ _ m0 m1 m2 H); eauto.
-Qed.
-
-(** These lemmas get rid of the unnecessary PER premises. *)
-Lemma per_sort_elem_pi' {P : PtsSig} {pred_P : PredicativeSig P} :
-  forall s_in s_out s_pi s (r : Ru_pi P s_in s_out s_pi) (sub : st_subtyp s_pi s) a a' Δ ρ B Δ' ρ' B'
-    (in_rel : relation (domain P))
-    (out_rel : forall {c c'} (equiv_c_c' : {{ Dom c ≈ c' ∈ in_rel }}), relation (domain P))
-    elem_rel,
-    {{ DF a ≈ a' ∈ per_sort_elem pred_P s_in ↘ in_rel}} ->
-    (forall {c c'} (equiv_c_c' : {{ Dom c ≈ c' ∈ in_rel }}),
-        rel_mod_eval (per_sort_elem pred_P s_out) B Δ d{{{ ρ ↦ c }}} B' Δ' d{{{ ρ' ↦ c' }}} (out_rel equiv_c_c')) ->
-    (elem_rel <~> fun f f' => forall c c' (equiv_c_c' : {{ Dom c ≈ c' ∈ in_rel }}), rel_mod_app f c f' c' (out_rel equiv_c_c')) ->
-    {{ DF Π r a (Δ ; ρ) B ≈ Π r a' (Δ' ; ρ') B' ∈ per_sort_elem pred_P s ↘ elem_rel }}.
-Proof.
-  intros.
-  per_sort_elem_econstructor'; eauto.
-  typeclasses eauto.
-Qed.
-
-Ltac per_sort_elem_econstructor :=
-  (repeat intro; hnf; (eapply per_sort_elem_pi')) + per_sort_elem_econstructor'.
-
-#[export]
-Hint Resolve per_sort_elem_pi' : mcpts.
-
-Lemma per_sort_elem_pi_clean_inversion {P : PtsSig} {pred_P : PredicativeSig P} : forall {s_in s_out s_pi s} {r : Ru_pi P s_in s_out s_pi} {sub : st_subtyp s_pi s} {a a' in_rel Δ Δ' ρ ρ' B B' elem_rel},
-    {{ DF a ≈ a' ∈ per_sort_elem pred_P s_in ↘ in_rel }} ->
-    {{ DF Π r a (Δ ; ρ) B ≈ Π r a' (Δ' ; ρ') B' ∈ per_sort_elem pred_P s ↘ elem_rel }} ->
-    exists (out_rel : forall {n n'} (equiv_n_n' : {{ Dom n ≈ n' ∈ in_rel }}), relation (domain P)),
-      (forall n n' (equiv_n_n' : {{ Dom n ≈ n' ∈ in_rel }}),
-          rel_mod_eval (per_sort_elem pred_P s_out) B Δ d{{{ ρ ↦ n }}} B' Δ' d{{{ ρ' ↦ n' }}} (out_rel equiv_n_n')) /\
-        (elem_rel <~> fun f f' => forall n n' (equiv_n_n' : {{ Dom n ≈ n' ∈ in_rel }}), rel_mod_app f n f' n' (out_rel equiv_n_n')).
-Proof.
-  intros * sub * Ha HΠ.
-  (unshelve eapply per_sort_elem_pi_left_inversion in HΠ; shelve_unifiable; deex_in HΠ; destruct HΠ as [_ [Heq [? []]]]; inversion Heq; subst).
-  rename a'0 into a'.
-  rename ρ'0 into ρ'.
-  rename B'0 into B'.
-  handle_per_sort_elem_irrel.
-  eexists.
-  split.
-  - instantiate (1 := fun n n' (equiv_n_n' : in_rel n n') m m' =>
-                        forall R,
-                          rel_typ pred_P s_out B Δ d{{{ ρ ↦ n }}} B' Δ'0 d{{{ ρ' ↦ n' }}} R ->
-                          R m m').
-    intros.
-    assert (in_rel0 n n') by intuition.
-    (on_all_hyp: destruct_rel_by_assumption in_rel0).
-    econstructor; eauto.
-    apply -> per_sort_elem_morphism_iff; eauto.
-    split; [| intuition].
-    intros.
-    destruct_by_head (@rel_typ P).
-    handle_per_sort_elem_irrel.
-    intuition.
-  - split; intros;
-      [assert (in_rel0 n n') by intuition; (on_all_hyp: destruct_rel_by_assumption in_rel0)
-      | assert (in_rel n n') by intuition; (on_all_hyp: destruct_rel_by_assumption in_rel)];
-      econstructor; intuition.
-    destruct_by_head (@rel_typ P).
-    handle_per_sort_elem_irrel.
-    intuition.
-Qed.
-
-Ltac invert_per_sort_elem H :=
-  (unshelve eapply (per_sort_elem_pi_clean_inversion _) in H; shelve_unifiable; [eassumption |]; destruct H as [? []])
-  + invert_per_sort_elem' H.
-
-Ltac invert_per_sort_elems := match_by_head per_sort_elem ltac:(fun H => directed invert_per_sort_elem H).
-
-
-Lemma per_sort_elem_cumu {P} {pred_P : PredicativeSig P} : forall s1 s2 a b R,
-    st_subtyp s1 s2 ->
-    {{ DF a ≈ b ∈ per_sort_elem pred_P s1 ↘ R }} ->
-    {{ DF a ≈ b ∈ per_sort_elem pred_P s2 ↘ R }}.
-Proof.
-  simpl.
-  induction 2 using per_sort_elem_ind; subst.
-  - eapply per_sort_elem_core_sort'; eauto.
-    transitivity s_elem; eauto.
-  - per_sort_elem_econstructor; eauto.    
-    + transitivity s_elem; eauto.
-    + intros.
-      destruct_rel_mod_eval.
-      econstructor; eauto.
-  - per_sort_elem_econstructor; eauto.
-    transitivity s_elem; mauto 2.
-  - per_sort_elem_econstructor; eauto.
-Qed.
-
-#[export]
-Hint Resolve per_sort_elem_cumu : mcpts.
- 
-Lemma per_subtyp_sorted_to_sort_elem {P} {pred_P : PredicativeSig P} : forall a b s,
-    {{ ⟪ pred_P ⟫ Subs a <: b at s }} ->
-    exists R R',
-      {{ DF a ≈ a ∈ per_sort_elem pred_P s ↘ R }} /\
-        {{ DF b ≈ b ∈ per_sort_elem pred_P s ↘ R' }}.
-Proof.
-  destruct 1;
-    match_by_head @per_sort ltac:(fun H => destruct H);
-    repeat eexists; mauto 2;
-    per_sort_elem_econstructor; try reflexivity;
-    etransitivity; try eassumption; symmetry; eassumption.
-Qed.
-
-Lemma per_elem_subtyping_sorted {P} {pred_P : PredicativeSig P} : forall A B s,
-    {{ ⟪ pred_P ⟫ Subs A <: B at s }} ->
-    forall R R' a b,
-      {{ DF A ≈ A ∈ per_sort_elem pred_P s ↘ R }} ->
-      {{ DF B ≈ B ∈ per_sort_elem pred_P s ↘ R' }} ->
-      R a b ->
-      R' a b.
-Proof.  
-  induction 1; intros;
-    match_by_head (@per_sort) ltac:(fun H => destruct H);
-    handle_per_sort_elem_irrel;
-    saturate_refl;
-    (on_all_hyp: fun H => directed invert_per_sort_elem H);
-    handle_per_sort_elem_irrel;
-    clear_refl_eqs;
-    trivial.
-  - unfold per_sort_rec in *.    
-    firstorder mauto.
-      
-  - intros.
-    destruct_conjs.
-    pose proof (ord_ru_pi_sub pred_P r sub1) as [ord_dom ord_im].
-    assert (per_sort_elem pred_P s1 in_rel1 a' a') by (destruct ord_dom; subst; mauto 2).
-    assert (per_sort_elem pred_P s1 in_rel0 a a) by (destruct ord_dom; subst; mauto 2).
-    handle_per_sort_elem_irrel.
-    assert (in_rel0 n n') as equiv0_n_n' by (apply_relation_equivalence; mauto 2).
-    clear ord_dom ord_im.
-    destruct_rel_mod_eval.
-    pose proof (ord_ru_pi_sub pred_P r sub1) as [ord_dom ord_im].
-    assert (per_sort_elem pred_P s2 (out_rel0 n n' equiv_n_n') a1 a'0) by (destruct ord_im; subst; mauto 2).
-    assert (per_sort_elem pred_P s2 (out_rel n n' equiv0_n_n') a2 a'1) by (destruct ord_im; subst; mauto 2).
-    saturate_refl_for (@per_sort_elem P).
-    clear ord_dom ord_im.
-    handle_per_sort_elem_irrel.    
-    destruct_rel_mod_app.
-    simplify_evals.
-    econstructor; intuition.
+  - pose proof (fun m m' => per_elem_sym _ _ _ _ _ m m' H); eauto.
+  - pose proof (fun m0 m1 m2 => per_elem_trans _ _ _ _ _ m0 m1 m2 H); eauto.
 Qed.
 
 
-Lemma per_elem_subtyping_sorted_gen {P} {pred_P : PredicativeSig P} : forall a b s a' b' R R' m n,
-    {{ ⟪ pred_P ⟫ Subs a <: b at s }} ->
-    {{ DF a ≈ a' ∈ per_sort_elem pred_P s ↘ R }} ->
-    {{ DF b ≈ b' ∈ per_sort_elem pred_P s ↘ R' }} ->
-    R m n ->
-    R' m n.
-Proof.
-  intros.
-  eapply per_elem_subtyping_sorted; saturate_refl; try eassumption.
-Qed.
 
-Lemma per_subtyp_sorted_refl1 {P} {pred_P : PredicativeSig P} : forall a b s R,
-    {{ DF a ≈ b ∈ per_sort_elem pred_P s ↘ R }} ->
-    {{ ⟪ pred_P ⟫ Subs a <: b at s }}.
-Proof.
-  simpl; induction 1 using per_sort_elem_ind;
-    subst;
-    mauto;
-    destruct_all.
-  - assert (st_subtyp s1' s1') by econstructor.
-    econstructor; mauto 4.    
-    
-  - assert ({{ DF Π r a (Δ ; ρ) B ≈ Π r a' (Δ' ; ρ') B' ∈ per_sort_elem pred_P s_elem ↘ elem_rel }})
-      by (per_sort_elem_econstructor; intuition; destruct_rel_mod_eval; mauto).
-    saturate_refl_for (@per_sort_elem P).
-    econstructor; eauto.
-    intros;
-      destruct_rel_mod_eval;
-      functional_eval_rewrite_clear;
-      trivial.
-  - econstructor; mauto 3.
-    eexists.
-    per_sort_elem_econstructor; eauto.
-Qed.
-
-#[export]
-Hint Resolve per_subtyp_sorted_refl1 : mcpts.
-
-Lemma per_subtyp_sorted_refl2 {P} {pred_P : PredicativeSig P} : forall a b s R,
-    {{ DF a ≈ b ∈ per_sort_elem pred_P s ↘ R }} ->
-    {{ ⟪ pred_P ⟫ Subs b <: a at s }}.
-Proof.
-  intros.
-  symmetry in H.
-  eauto using per_subtyp_sorted_refl1.
-Qed.
-
-#[export]
-Hint Resolve per_subtyp_sorted_refl2 : mcpts.
-
-Lemma per_subtyp_sorted_trans {P} {pred_P : PredicativeSig P} : forall a1 a2 s,
-    {{ ⟪ pred_P ⟫ Subs a1 <: a2 at s }} ->
-    forall a3,
-      {{ ⟪ pred_P ⟫ Subs a2 <: a3 at s }} ->
-      {{ ⟪ pred_P ⟫ Subs a1 <: a3 at s }}.
-Proof.
-  induction 1; intros ? Hsub; simpl in *.
-  (* Universe, nat and neutral cases *)
-  1,2,4: progressive_inversion; mauto.
-  - econstructor; mauto 2.
-    transitivity s2; mauto 2.
-  - dependent destruction Hsub; subst.
-    handle_per_sort_elem_irrel.
-    econstructor; eauto.
-    + etransitivity; eassumption.
-    + intros.
-      saturate_refl_for (@per_sort_elem P).
-      saturate_refl_for in_rel0.
-      (on_all_hyp: fun H => directed invert_per_sort_elem H).
-      destruct_conjs.
-      assert (per_sort_elem pred_P s1 in_rel a a).
-      {
-        pose proof (ord_ru_pi_sub pred_P r sub) as [ord_dom ord_im].
-        destruct ord_dom; subst; mauto 2.
-      }
-      assert (per_sort_elem pred_P s1 in_rel1 a' a').
-      {
-        pose proof (ord_ru_pi_sub pred_P r sub) as [ord_dom ord_im].
-        destruct ord_dom; subst; mauto 2.
-      }
-      assert (per_sort_elem pred_P s1 in_rel2 a'0 a'0).
-      {
-        pose proof (ord_ru_pi_sub pred_P r sub) as [ord_dom ord_im].
-        destruct ord_dom; subst; mauto 2.
-      }
-      handle_per_sort_elem_irrel.
-      destruct_rel_mod_eval.
-      handle_per_sort_elem_irrel.
-      assert (per_sort_elem pred_P s2 (out_rel1 c' c' H19) b' b').
-      {
-        pose proof (ord_ru_pi_sub pred_P r sub2) as [ord_dom ord_im].
-        destruct ord_im; subst; mauto 2.
-      }
-      assert (per_sort_elem pred_P s2 (out_rel1 c c' H13) a1 b').
-      {
-        pose proof (ord_ru_pi_sub pred_P r sub2) as [ord_dom ord_im].
-        destruct ord_im; subst; mauto 2.
-      }
-      assert (per_sort_elem pred_P s2 (out_rel1 c c H18) a1 a1).
-      {
-        pose proof (ord_ru_pi_sub pred_P r sub2) as [ord_dom ord_im].
-        destruct ord_im; subst; mauto 2.
-      }
-      handle_per_sort_elem_irrel.
-      assert (in_rel c c') by intuition. 
-      assert (in_rel1 c c') by intuition.
-      assert (PER in_rel).
-      {
-        split.
-        - intros x y Hxy.
-          eapply H29 in Hxy.
-          eapply H29.
-          symmetry.
-          eassumption.
-        - intros x y z Hxy Hyz.
-          eapply H29.
-          eapply H29 in Hxy.
-          eapply H29 in Hyz.
-          transitivity y; eassumption.
-      }
-      saturate_refl_for in_rel.
-      saturate_refl_for in_rel1.
-      destruct_rel_mod_eval.
-      simplify_evals.
-      
-      assert {{ ⟪ pred_P ⟫ Subs b <: a5 at s2 }} by (eapply (H0 c c); mauto 3).
-      assert {{ ⟪ pred_P ⟫ Subs a5 <: b' at s2 }} by (eapply (H6 c c'); mauto 3).
-      eapply (H1 c c'); mauto 3.
-Qed.
-
-#[export]
-Hint Resolve per_subtyp_sorted_trans : mcpts.
-
-#[export]
-Instance per_subtyp_sorted_trans_ins {P} {pred_P : PredicativeSig P} s : Transitive (per_subtyp_sorted pred_P s).
-Proof.
-  eauto using per_subtyp_sorted_trans.
-Qed.
-
-Lemma per_subtyp_sorted_transp {P} {pred_P : PredicativeSig P} : forall a b s a' b' R R',
-    {{ ⟪ pred_P ⟫ Subs a <: b at s }} ->
-    {{ DF a ≈ a' ∈ per_sort_elem pred_P s ↘ R }} ->
-    {{ DF b ≈ b' ∈ per_sort_elem pred_P s ↘ R' }} ->
-    {{ ⟪ pred_P ⟫ Subs a' <: b' at s }}.
-Proof.
-  mauto using per_subtyp_sorted_refl1, per_subtyp_sorted_refl2.
-Qed.
-
-Lemma per_subtyp_sorted_cumu {P} {pred_P : PredicativeSig P} : forall a1 a2 s,
-    {{ ⟪ pred_P ⟫ Subs a1 <: a2 at s }} ->
-    forall s',
-      st_subtyp s s' ->
-      {{ ⟪ pred_P ⟫ Subs a1 <: a2 at s' }}.
-Proof.
-  induction 1; intros; econstructor; mauto;
-    match_by_head (@per_sort P) ltac:(fun H => destruct H);
-    only 4: (etransitivity; eassumption);
-    eexists; mauto 2.
-Qed.
-
-#[export]
-Hint Resolve per_subtyp_sorted_cumu : mcpts.
-
-
-(** Lemmas for per_typ_elem and per_typ *)
-Add Parametric Morphism {P : PtsSig} {pred_P : PredicativeSig P} : (per_typ_elem pred_P)
-  with signature (@relation_equivalence (domain P)) ==> eq ==> eq ==> iff as per_typ_elem_morphism_iff.
-Proof with mautosolve.
-  intros R R' HRR'.
-  split; intro Horig; [gen R' | gen R];
-    induction Horig; econstructor;
-    apply_relation_equivalence; try reflexivity; try eassumption.
-Qed.
-
-Add Parametric Morphism {P : PtsSig} {pred_P : PredicativeSig P} : (per_typ_elem pred_P)
-  with signature (@relation_equivalence (domain P)) ==> (@relation_equivalence (domain P)) as per_typ_elem_morphism_relation_equivalence.
-Proof.
-  intros * H ? ?.
-  simpl.
-  rewrite H.
-  reflexivity.
-Qed.
-
-Lemma per_typ_elem_right_irrel {P : PtsSig} {pred_P : PredicativeSig P} : forall a b b' R R',
-    {{ DF a ≈ b ∈ per_typ_elem pred_P ↘ R }} ->
-    {{ DF a ≈ b' ∈ per_typ_elem pred_P ↘ R' }} ->
+Lemma per_typ_elem_right_irrel {P : PtsSig} {pred_P : PredicativeSig P} : forall Δ a b b' R R',
+    {{ DF a ≈ b ∈ per_typ_elem pred_P Δ ↘ R }} ->
+    {{ DF a ≈ b' ∈ per_typ_elem pred_P Δ ↘ R' }} ->
     R <~> R'.
 Proof.
   intros * Horig.
@@ -1020,9 +740,9 @@ Proof.
 Qed.
 
 
-Lemma per_typ_elem_sym {P} {pred_P : PredicativeSig P} : forall {R a b},
-    {{ DF a ≈ b ∈ per_typ_elem pred_P ↘ R }} ->
-    {{ DF b ≈ a ∈ per_typ_elem pred_P ↘ R }} /\
+Lemma per_typ_elem_sym {P} {pred_P : PredicativeSig P} : forall {Δ R a b},
+    {{ DF a ≈ b ∈ per_typ_elem pred_P Δ ↘ R }} ->
+    {{ DF b ≈ a ∈ per_typ_elem pred_P Δ ↘ R }} /\
       (forall m m',
           {{ Dom m ≈ m' ∈ R }} ->
           {{ Dom m' ≈ m ∈ R }}).
@@ -1033,15 +753,15 @@ Proof with mautosolve.
   - apply_relation_equivalence.
     intros.
     eapply per_sort_sym'; mauto.
-  - assert {{ DF b ≈ a ∈ per_sort_elem pred_P s ↘ R }} by (eapply per_sort_sym; mauto).
+  - assert {{ DF b ≈ a ∈ per_sort_elem pred_P Δ s ↘ R }} by (eapply per_sort_sym; mauto).
     econstructor; mauto.
   - intros.
     eapply per_elem_sym; mauto.
 Qed.
 
-Corollary per_typ_elem_left_irrel {P} {pred_P : PredicativeSig P} : forall R a b R' a',
-    {{ DF a ≈ b ∈ per_typ_elem pred_P ↘ R }} ->
-    {{ DF a' ≈ b ∈ per_typ_elem pred_P ↘ R' }} ->
+Corollary per_typ_elem_left_irrel {P} {pred_P : PredicativeSig P} : forall Δ R a b R' a',
+    {{ DF a ≈ b ∈ per_typ_elem pred_P Δ ↘ R }} ->
+    {{ DF a' ≈ b ∈ per_typ_elem pred_P Δ ↘ R' }} ->
     R <~> R'.
 Proof.
   intros * ?%per_typ_elem_sym ?%per_typ_elem_sym.
@@ -1049,9 +769,9 @@ Proof.
   eauto using per_typ_elem_right_irrel.
 Qed.
 
-Corollary per_typ_elem_cross_irrel {P} {pred_P : PredicativeSig P} : forall R a b R' b',
-    {{ DF a ≈ b ∈ per_typ_elem pred_P ↘ R }} ->
-    {{ DF b' ≈ a ∈ per_typ_elem pred_P ↘ R' }} ->
+Corollary per_typ_elem_cross_irrel {P} {pred_P : PredicativeSig P} : forall Δ R a b R' b',
+    {{ DF a ≈ b ∈ per_typ_elem pred_P Δ ↘ R }} ->
+    {{ DF b' ≈ a ∈ per_typ_elem pred_P Δ ↘ R' }} ->
     R <~> R'.
 Proof.
   intros * ? ?%per_typ_elem_sym.
@@ -1062,24 +782,24 @@ Qed.
 Ltac do_per_typ_elem_irrel_assert1 :=
   let tactic_error o1 o2 := fail 2 "per_typ_elem_irrel biconditional between" o1 "and" o2 "cannot be solved" in
   match goal with
-  | H1 : {{ DF ^?a ≈ ^_ ∈ per_typ_elem ?pred_P ↘ ?R1 }},
-      H2 : {{ DF ^?a ≈ ^_ ∈ per_typ_elem ?pred_P ↘ ?R2 }} |- _ =>
+  | H1 : {{ DF ^?a ≈ ^_ ∈ per_typ_elem ?pred_P ?Δ ↘ ?R1 }},
+      H2 : {{ DF ^?a ≈ ^_ ∈ per_typ_elem ?pred_P ?Δ ↘ ?R2 }} |- _ =>
       assert_fails (unify R1 R2);
       match goal with
       | H : R1 <~> R2 |- _ => fail 1
       | H : R2 <~> R1 |- _ => fail 1
       | _ => assert (R1 <~> R2) by (eapply per_typ_elem_right_irrel; [apply H1 | apply H2]) || tactic_error R1 R2
       end
-  | H1 : {{ DF ^_ ≈ ^?b ∈ per_typ_elem ?pred_P ↘ ?R1 }},
-      H2 : {{ DF ^_ ≈ ^?b ∈ per_typ_elem ?pred_P ↘ ?R2 }} |- _ =>
+  | H1 : {{ DF ^_ ≈ ^?b ∈ per_typ_elem ?pred_P ?Δ ↘ ?R1 }},
+      H2 : {{ DF ^_ ≈ ^?b ∈ per_typ_elem ?pred_P ?Δ ↘ ?R2 }} |- _ =>
       assert_fails (unify R1 R2);
       match goal with
       | H : R1 <~> R2 |- _ => fail 1
       | H : R2 <~> R1 |- _ => fail 1
       | _ => assert (R1 <~> R2) by (eapply per_typ_elem_left_irrel; [apply H1 | apply H2]) || tactic_error R1 R2
       end
-  | H1 : {{ DF ^?a ≈ ^_ ∈ per_typ_elem ?pred_P ↘ ?R1 }},
-      H2 : {{ DF ^_ ≈ ^?a ∈ per_typ_elem ?pred_P ↘ ?R2 }} |- _ =>
+  | H1 : {{ DF ^?a ≈ ^_ ∈ per_typ_elem ?pred_P ?Δ ↘ ?R1 }},
+      H2 : {{ DF ^_ ≈ ^?a ∈ per_typ_elem ?pred_P ?Δ ↘ ?R2 }} |- _ =>
       (** Order matters less here as H1 and H2 cannot be exchanged *)
       assert_fails (unify R1 R2);
       match goal with
@@ -1098,12 +818,11 @@ Ltac handle_per_typ_elem_irrel :=
   apply_relation_equivalence;
   clear_dups.
 
-
-Lemma per_typ_elem_trans {P} {pred_P : PredicativeSig P} : forall R a1 a2,
-    {{ DF a1 ≈ a2 ∈ per_typ_elem pred_P ↘ R }} ->
+Lemma per_typ_elem_trans {P} {pred_P : PredicativeSig P} : forall Δ R a1 a2,
+    {{ DF a1 ≈ a2 ∈ per_typ_elem pred_P Δ ↘ R }} ->
     (forall a3,
-        {{ DF a2 ≈ a3 ∈ per_typ_elem pred_P ↘ R }} ->
-        {{ DF a1 ≈ a3 ∈ per_typ_elem pred_P ↘ R }}) /\
+        {{ DF a2 ≈ a3 ∈ per_typ_elem pred_P Δ ↘ R }} ->
+        {{ DF a1 ≈ a3 ∈ per_typ_elem pred_P Δ ↘ R }}) /\
       (forall m1 m2 m3,
           R m1 m2 ->
           R m2 m3 ->
@@ -1121,44 +840,43 @@ Proof with mautosolve.
       dependent destruction H0.
       * apply_relation_equivalence.
         econstructor; mauto.
-      * assert {{ DF a ≈ b ∈ per_sort_elem pred_P s ↘ R }} by (eapply per_sort_trans; mauto).
+      * assert {{ DF a ≈ b ∈ per_sort_elem pred_P Δ s ↘ R }} by (eapply per_sort_trans; mauto).
         econstructor; mauto.
-    + apply_relation_equivalence.
-      eapply per_sort_elem_trans; mauto.
+    + eapply per_sort_elem_trans; mauto.
 Qed.
 
 #[export]
-Instance per_typ_elem_PER {P} {pred_P : PredicativeSig P} {R} : PER (per_typ_elem pred_P R).
+Instance per_typ_elem_PER {P} {pred_P : PredicativeSig P} {Δ R} : PER (per_typ_elem pred_P Δ R).
 Proof.
   split.
   - intros x y H.
     eapply (per_typ_elem_sym H).
   - intros x y **.
-    eapply (per_typ_elem_trans R x y ltac:(eassumption)); eassumption.
+    eapply (per_typ_elem_trans Δ R x _ ltac:(eassumption)); eassumption.
 Qed.
 
 
-Corollary per_typ_sym {P} {pred_P : PredicativeSig P} : forall a b,
-    {{ Dom a ≈ b ∈ per_typ pred_P }} ->
-    {{ Dom b ≈ a ∈ per_typ pred_P }}.
+Corollary per_typ_sym {P} {pred_P : PredicativeSig P} : forall Δ a b,
+    {{ Dom a ≈ b ∈ per_typ pred_P Δ }} ->
+    {{ Dom b ≈ a ∈ per_typ pred_P Δ }}.
 Proof.
   intros * [? ?%per_typ_elem_sym].
   firstorder.
 Qed.
 
-Corollary per_typ_trans {P : PtsSig} {pred_P : PredicativeSig P} : forall a1 a2 a3,
-    {{ Dom a1 ≈ a2 ∈ per_typ pred_P }} ->
-    {{ Dom a2 ≈ a3 ∈ per_typ pred_P }} ->
-    {{ Dom a1 ≈ a3 ∈ per_typ pred_P }}.
+Corollary per_typ_trans {P : PtsSig} {pred_P : PredicativeSig P} : forall Δ a1 a2 a3,
+    {{ Dom a1 ≈ a2 ∈ per_typ pred_P Δ }} ->
+    {{ Dom a2 ≈ a3 ∈ per_typ pred_P Δ }} ->
+    {{ Dom a1 ≈ a3 ∈ per_typ pred_P Δ }}.
 Proof.
   intros * [? ?] [? ?].
   handle_per_typ_elem_irrel.
-  assert (per_typ_elem pred_P x0 a1 a3) by (eapply (proj1 (per_typ_elem_trans x0 a1 a2 H) a3 H0); mauto).
+  assert (per_typ_elem pred_P Δ x0 a1 a3) by (eapply (proj1 (per_typ_elem_trans Δ x0 a1 a2 H) a3 H0); mauto).
   mauto.
 Qed.
 
 #[export]
-Instance per_typ_PER {P} {pred_P : PredicativeSig P} : PER (per_typ pred_P).
+Instance per_typ_PER {P} {pred_P : PredicativeSig P} {Δ} : PER (per_typ pred_P Δ).
 Proof.
   split.
   - intros x y H.
@@ -1167,6 +885,371 @@ Proof.
     eapply per_typ_trans; mauto.
 Qed.
 
+
+Lemma per_typ_elem_and_per_sort_elem_implies_per_sort_elem {P} (pred_P : PredicativeSig P) : forall {Δ a b c R R' s},
+    {{ DF a ≈ b ∈ per_typ_elem pred_P Δ ↘ R }} ->
+    {{ DF a ≈ c ∈ per_sort_elem pred_P Δ s ↘ R' }} ->
+    {{ DF a ≈ b ∈ per_sort_elem pred_P Δ s ↘ R }}.
+Proof.
+  intros * Hab.
+  inversion_clear Hab; intros.
+  - basic_invert_per_sort_elem H0; mauto.
+  - handle_per_sort_elem_irrel.
+    assert (per_sort_elem pred_P Δ s R c a) by (eapply (per_sort_elem_sym H0); mauto).
+    assert (per_sort_elem pred_P Δ s R c b) by (eapply (per_sort_elem_trans Δ s R c a H1); eassumption).
+    eapply (per_sort_elem_trans Δ s R a c H0); eassumption.
+Qed.
+
+#[export]
+Hint Resolve per_typ_elem_and_per_sort_elem_implies_per_sort_elem : mcpts.
+
+
+(** These lemmas get rid of the unnecessary PER premises. *)
+Lemma per_sort_elem_pi' {P : PtsSig} {pred_P : PredicativeSig P} :
+  forall Δ s_in s_out s_pi s (r : Ru_pi P s_in s_out s_pi) (sub : st_subtyp s_pi s) a a' ρ B ρ' B'
+    (in_rel : relation (domain P))
+    (out_rel : forall {c c'} (equiv_c_c' : {{ Dom c ≈ c' ∈ in_rel }}), relation (domain P))
+    elem_rel,
+    {{ DF a ≈ a' ∈ per_sort_elem pred_P Δ s_in ↘ in_rel}} ->
+    (forall {c c'} (equiv_c_c' : {{ Dom c ≈ c' ∈ in_rel }}),
+        rel_mod_eval (per_sort_elem pred_P Δ s_out) Δ B d{{{ ρ ↦ c }}} B' d{{{ ρ' ↦ c' }}} (out_rel equiv_c_c')) ->
+    (elem_rel <~> fun f f' => forall c c' (equiv_c_c' : {{ Dom c ≈ c' ∈ in_rel }}), rel_mod_app Δ f c f' c' (out_rel equiv_c_c')) ->
+    {{ DF Π r a ρ B ≈ Π r a' ρ' B' ∈ per_sort_elem pred_P Δ s ↘ elem_rel }}.
+Proof.
+  intros.
+  per_sort_elem_econstructor'; eauto.
+  typeclasses eauto.
+Qed.
+
+Ltac per_sort_elem_econstructor :=
+  (repeat intro; hnf; (eapply per_sort_elem_pi')) + per_sort_elem_econstructor'.
+
+#[export]
+Hint Resolve per_sort_elem_pi' : mcpts.
+
+Lemma per_sort_elem_pi_clean_inversion {P : PtsSig} {pred_P : PredicativeSig P} : forall {Δ s_in s_out s_pi s} {r : Ru_pi P s_in s_out s_pi} {sub : st_subtyp s_pi s} {a a' in_rel ρ ρ' B B' elem_rel},
+    {{ DF a ≈ a' ∈ per_sort_elem pred_P Δ s_in ↘ in_rel }} ->
+    {{ DF Π r a ρ B ≈ Π r a' ρ' B' ∈ per_sort_elem pred_P Δ s ↘ elem_rel }} ->
+    exists (out_rel : forall {n n'} (equiv_n_n' : {{ Dom n ≈ n' ∈ in_rel }}), relation (domain P)),
+      (forall n n' (equiv_n_n' : {{ Dom n ≈ n' ∈ in_rel }}),
+          rel_mod_eval (per_sort_elem pred_P Δ s_out) Δ B d{{{ ρ ↦ n }}} B' d{{{ ρ' ↦ n' }}} (out_rel equiv_n_n')) /\
+        (elem_rel <~> fun f f' => forall n n' (equiv_n_n' : {{ Dom n ≈ n' ∈ in_rel }}), rel_mod_app Δ f n f' n' (out_rel equiv_n_n')).
+Proof.
+  intros * sub * Ha HΠ.
+  (unshelve eapply per_sort_elem_pi_left_inversion in HΠ; shelve_unifiable; deex_in HΠ; destruct HΠ as [_ [Heq [? []]]]; inversion Heq; subst).
+  rename a'0 into a'.
+  rename ρ'0 into ρ'.
+  rename B'0 into B'.
+  handle_per_sort_elem_irrel.
+  eexists.
+  split.
+  - instantiate (1 := fun n n' (equiv_n_n' : in_rel n n') m m' =>
+                        forall R,
+                          rel_typ_unsorted pred_P Δ B d{{{ ρ ↦ n }}} B' d{{{ ρ' ↦ n' }}} R ->
+                          R m m').
+    intros.
+    assert (in_rel0 n n') by intuition.
+    (on_all_hyp: destruct_rel_by_assumption in_rel0).
+    econstructor; eauto.
+    apply -> per_sort_elem_morphism_iff; eauto.
+    split.
+    + intros.
+      destruct_by_head (@rel_typ_unsorted).
+      simplify_evals.
+      assert (per_sort_elem pred_P Δ s_out R a0 a'0) by mauto 2.
+      handle_per_sort_elem_irrel.
+      intuition.
+    + intuition.
+      eapply H6.
+      econstructor; mauto 3.
+  - split; intros;
+      [assert (in_rel0 n n') by intuition; (on_all_hyp: destruct_rel_by_assumption in_rel0)
+      | assert (in_rel n n') by intuition; (on_all_hyp: destruct_rel_by_assumption in_rel)];
+      econstructor; intuition.
+    + destruct_by_head (@rel_typ_unsorted P).
+      simplify_evals.
+      assert (per_sort_elem pred_P Δ s_out R a0 a'0) by mauto 2.
+      handle_per_sort_elem_irrel.
+      intuition.
+    + destruct_rel_mod_app.
+      destruct_rel_mod_eval.
+      simplify_evals.
+      eapply H9.
+      econstructor; mauto 3.
+Qed.
+
+Ltac invert_per_sort_elem H :=
+  (unshelve eapply (per_sort_elem_pi_clean_inversion _) in H; shelve_unifiable; [eassumption |]; destruct H as [? []])
+  + invert_per_sort_elem' H.
+
+Ltac invert_per_sort_elems := match_by_head per_sort_elem ltac:(fun H => directed invert_per_sort_elem H).
+
+
+Lemma per_sort_elem_pi_lowering {P} (pred_P : PredicativeSig P) : forall {Δ s1 s2 s3 s} {r : Ru_pi P s1 s2 s3} {elem_rel a ρ B a' ρ' B'},
+    {{ DF Π r a ρ B ≈ Π r a' ρ' B' ∈ per_sort_elem pred_P Δ s ↘ elem_rel }} ->
+    {{ DF Π r a ρ B ≈ Π r a' ρ' B' ∈ per_sort_elem pred_P Δ s3 ↘ elem_rel }}.
+Proof.
+  intros.
+  invert_per_sort_elem H.
+  per_sort_elem_econstructor; mauto 3.
+  - destruct_conjs.
+    pose proof ord_ru_pi_sub pred_P r sub as [[] ?]; subst; mauto 2.
+  - intros.
+    destruct_rel_mod_eval.
+    econstructor; mauto 3.
+    pose proof ord_ru_pi_sub pred_P r sub as [? []]; subst; mauto 2.
+Qed.
+
+Lemma per_typ_elem_pi_lowering {P} (pred_P : PredicativeSig P) : forall {Δ s1 s2 s3} {r : Ru_pi P s1 s2 s3} {elem_rel a ρ B a' ρ' B'},
+    {{ DF Π r a ρ B ≈ Π r a' ρ' B' ∈ per_typ_elem pred_P Δ ↘ elem_rel }} ->
+    {{ DF Π r a ρ B ≈ Π r a' ρ' B' ∈ per_sort_elem pred_P Δ s3 ↘ elem_rel }}.
+Proof.
+  intros.
+  inversion_clear H.
+  eapply per_sort_elem_pi_lowering; mauto 2.
+Qed.
+
+
+Lemma per_sort_elem_cumu {P} {pred_P : PredicativeSig P} : forall Δ s1 s2 a b R,
+    st_subtyp s1 s2 ->
+    {{ DF a ≈ b ∈ per_sort_elem pred_P Δ s1 ↘ R }} ->
+    {{ DF a ≈ b ∈ per_sort_elem pred_P Δ s2 ↘ R }}.
+Proof.
+  simpl.
+  induction 2 using per_sort_elem_ind; subst.
+  - eapply per_sort_elem_core_sort'; eauto.
+    transitivity s_elem; eauto.
+  - per_sort_elem_econstructor; eauto.    
+    + transitivity s_elem; eauto.
+    + intros.
+      destruct_rel_mod_eval.
+      econstructor; eauto.
+  - per_sort_elem_econstructor; eauto.
+    transitivity s_elem; mauto 2.
+  - per_sort_elem_econstructor; eauto.
+Qed.
+
+#[export]
+Hint Resolve per_sort_elem_cumu : mcpts.
+
+
+
+
+(** * Lemmas related to semantic subtyping *)
+Lemma per_subtyp_sorted_to_sort_elem {P} {pred_P : PredicativeSig P} : forall Δ a b,
+    (exists s : P, True) ->
+    {{ SubT a <: b ∈ per_subtyp pred_P Δ }} ->
+    (* {{ ⟪ pred_P ⟫ Subs a <: b at s }} -> *)
+    exists R R',
+      {{ DF a ≈ a ∈ per_typ_elem pred_P Δ ↘ R }} /\
+        {{ DF b ≈ b ∈ per_typ_elem pred_P Δ ↘ R' }}.
+Proof.
+  intros * [s] [].
+  - repeat eexists; econstructor; reflexivity.
+  - repeat eexists; econstructor;
+      per_sort_elem_econstructor; mauto 2; reflexivity.
+  - repeat eexists; econstructor; try eassumption.
+  - repeat eexists;
+      unshelve econstructor; try eassumption; shelve_unifiable;
+      per_sort_elem_econstructor; mauto 2; try reflexivity;
+      etransitivity; try eassumption; symmetry; eassumption.
+Qed.
+
+Lemma per_elem_subtyping {P} {pred_P : PredicativeSig P} : forall Δ a b,
+    {{ SubT a <: b ∈ per_subtyp pred_P Δ }} ->
+    forall R R' m n,
+      {{ DF a ≈ a ∈ per_typ_elem pred_P Δ ↘ R }} ->
+      {{ DF b ≈ b ∈ per_typ_elem pred_P Δ ↘ R' }} ->
+      R m n ->
+      R' m n.
+Proof.
+  induction 1; intros * Ha Hb.
+  - assert (per_typ_elem pred_P Δ (per_sort pred_P Δ s1) d{{{ Sort@s1 }}} d{{{ Sort@s1 }}}) by (econstructor; try reflexivity).
+    assert (per_typ_elem pred_P Δ (per_sort pred_P Δ s2) d{{{ Sort@s2 }}} d{{{ Sort@s2 }}}) by (econstructor; try reflexivity).
+    handle_per_typ_elem_irrel.
+    unfold per_sort; intros [R].
+    assert (per_sort_elem pred_P Δ s2 R m n) by mauto 2.
+    mauto 2.
+
+  - inversion_clear Ha; inversion_clear Hb.
+    handle_per_sort_elem_irrel.
+    mauto 2.
+  - saturate_refl.
+    assert (per_typ_elem pred_P Δ elem_rel d{{{ Π r a ρ B }}} d{{{ Π r a ρ B }}}) by mauto 2.
+    assert (per_typ_elem pred_P Δ elem_rel' d{{{ Π r a' ρ' B' }}} d{{{ Π r a' ρ' B' }}}) by mauto 2.
+    handle_per_typ_elem_irrel.    
+    invert_per_sort_elems.
+    destruct_conjs.
+    assert (per_sort_elem pred_P Δ s1 in_rel0 a a) by (pose proof ord_ru_pi_sub pred_P r sub0 as [[] ?]; subst; mauto 2).
+    assert (per_sort_elem pred_P Δ s1 in_rel1 a' a') by (pose proof ord_ru_pi_sub pred_P r sub0 as [[] ?]; subst; mauto 2).    
+    handle_per_sort_elem_irrel.
+
+    intros.
+    rename equiv_n_n' into equiv0_n0_n'.
+    assert (in_rel0 n0 n') as equiv_n0_n' by intuition.    
+    destruct_rel_mod_eval.
+    assert (per_sort_elem pred_P Δ s2 (out_rel0 n0 n' equiv0_n0_n') a0 a'0) by (pose proof ord_ru_pi_sub pred_P r sub1 as [? []]; subst; mauto 2).
+    assert (per_sort_elem pred_P Δ s2 (out_rel n0 n' equiv_n0_n') a1 a'1) by (pose proof ord_ru_pi_sub pred_P r sub1 as [? []]; subst; mauto 2).
+    saturate_refl_for (@per_sort_elem P).
+
+    destruct_rel_mod_app.
+    econstructor; mauto 2.
+    eapply H1; mauto 2.
+    
+  - inversion_clear Ha; inversion_clear Hb.
+    invert_per_sort_elems.
+    apply_relation_equivalence.
+    mauto 2.
+Qed.
+
+
+Lemma per_elem_subtyping_gen {P} {pred_P : PredicativeSig P} : forall Δ a b a' b' R R' m n,
+    {{ SubT a <: b ∈ per_subtyp pred_P Δ }} ->
+    {{ DF a ≈ a' ∈ per_typ_elem pred_P Δ ↘ R }} ->
+    {{ DF b ≈ b' ∈ per_typ_elem pred_P Δ ↘ R' }} ->
+    R m n ->
+    R' m n.
+Proof.
+  intros.
+  eapply per_elem_subtyping; saturate_refl; try eassumption.
+Qed.
+
+Lemma per_subtyp_sorted_refl1 {P} {pred_P : PredicativeSig P} : forall Δ s a b R,
+    {{ DF a ≈ b ∈ per_sort_elem pred_P Δ s ↘ R }} ->
+    {{ SubT a <: b ∈ per_subtyp pred_P Δ }}.
+Proof.  
+  simpl; induction 1 using per_sort_elem_ind;
+    subst;
+    mauto;
+    destruct_all.
+  - assert ({{ DF Π r a ρ B ≈ Π r a' ρ' B' ∈ per_sort_elem pred_P Δ s_elem ↘ elem_rel }})
+      by (per_sort_elem_econstructor; intuition; destruct_rel_mod_eval; mauto).
+    saturate_refl_for (@per_sort_elem P).
+    econstructor; eauto.
+    intros;
+      destruct_rel_mod_eval;
+      functional_eval_rewrite_clear;
+      trivial.
+Qed.
+
+#[export]
+Hint Resolve per_subtyp_sorted_refl1 : mcpts.
+
+Lemma per_subtyp_sorted_refl2 {P} {pred_P : PredicativeSig P} : forall Δ s a b R,
+    {{ DF a ≈ b ∈ per_sort_elem pred_P Δ s ↘ R }} ->
+    {{ SubT b <: a ∈ per_subtyp pred_P Δ }}.
+Proof.
+  intros.
+  symmetry in H.
+  eauto using per_subtyp_sorted_refl1.
+Qed.
+
+#[export]
+Hint Resolve per_subtyp_sorted_refl2 : mcpts.
+
+Lemma per_subtyp_refl1 {P} {pred_P : PredicativeSig P} : forall Δ a b R,
+    {{ DF a ≈ b ∈ per_typ_elem pred_P Δ ↘ R }} ->
+    {{ SubT a <: b ∈ per_subtyp pred_P Δ }}.
+Proof.
+  destruct 1.
+  - econstructor; reflexivity.
+  - eapply per_subtyp_sorted_refl1; mauto 2.
+Qed.
+
+#[export]
+Hint Resolve per_subtyp_refl1 : mcpts.
+
+Lemma per_subtyp_refl2 {P} {pred_P : PredicativeSig P} : forall Δ a b R,
+    {{ DF a ≈ b ∈ per_typ_elem pred_P Δ ↘ R }} ->
+    {{ SubT b <: a ∈ per_subtyp pred_P Δ }}.
+Proof.
+  intros.
+  symmetry in H.
+  eauto using per_subtyp_refl1.
+Qed.
+
+#[export]
+Hint Resolve per_subtyp_refl2 : mcpts.
+
+Lemma per_subtyp_trans {P} {pred_P : PredicativeSig P} : forall Δ a1 a2,
+    {{ SubT a1 <: a2 ∈ per_subtyp pred_P Δ }} ->
+    forall a3,
+      {{ SubT a2 <: a3 ∈ per_subtyp pred_P Δ }} ->
+      {{ SubT a1 <: a3 ∈ per_subtyp pred_P Δ }}.
+Proof.
+  induction 1; intros ? Hsub; simpl in *.
+  1,2,4: progressive_inversion; mauto.
+  - econstructor; mauto 2.
+    transitivity s2; mauto 2.
+  - dependent destruction Hsub; subst.
+    handle_per_sort_elem_irrel.
+    unshelve econstructor; only 4: auto; shelve_unifiable; eauto.
+    + etransitivity; eassumption.
+    + intros.
+      saturate_refl_for (@per_sort_elem P).
+      saturate_refl_for in_rel0.
+      (on_all_hyp: fun H => directed invert_per_sort_elem H).
+      destruct_conjs.
+      assert (per_sort_elem pred_P Δ s1 in_rel a a) by (pose proof ord_ru_pi_sub pred_P r sub as [[] ?]; subst; mauto 2).
+      assert (per_sort_elem pred_P Δ s1 in_rel1 a' a') by (pose proof ord_ru_pi_sub pred_P r sub as [[] ?]; subst; mauto 2).
+      assert (per_sort_elem pred_P Δ s1 in_rel2 a' a') by (pose proof ord_ru_pi_sub pred_P r sub2 as [[] ?]; subst; mauto 2).
+      assert (per_sort_elem pred_P Δ s1 in_rel3 a'0 a'0) by (pose proof ord_ru_pi_sub pred_P r sub2 as [[] ?]; subst; mauto 2).
+      handle_per_sort_elem_irrel.
+      rename H21 into equiv3_c_c, H22 into equiv3_c'_c'.
+      assert (in_rel c c) as equiv_c_c by intuition.
+      assert (in_rel1 c c) as equiv1_c_c by intuition.
+      assert (in_rel2 c c) as equiv2_c_c by intuition.
+      assert (in_rel c' c') as equiv_c'_c' by intuition.
+      assert (in_rel1 c' c') as equiv1_c'_c' by intuition.
+      assert (in_rel2 c' c') as equiv2_c'_c' by intuition.
+      destruct_rel_mod_eval.
+      simplify_evals.
+
+      assert (per_subtyp pred_P Δ b a3) by mauto 2.
+      assert (per_subtyp pred_P Δ a3 b') by mauto 2.
+      eapply (H1 c c' b a3); mauto 2.
+    + pose proof (per_sort_elem_pi_lowering pred_P H2).
+      mauto 2.
+Qed.
+
+#[export]
+Hint Resolve per_subtyp_trans : mcpts.
+
+#[export]
+Instance per_subtyp_trans_ins {P} {pred_P : PredicativeSig P} {Δ} : Transitive (per_subtyp pred_P Δ).
+Proof.
+  eauto using per_subtyp_trans.
+Qed.
+
+Lemma per_subtyp_transp {P} {pred_P : PredicativeSig P} : forall Δ a b a' b' R R',
+    {{ SubT a <: b ∈ per_subtyp pred_P Δ }} ->
+    {{ DF a ≈ a' ∈ per_typ_elem pred_P Δ ↘ R }} ->
+    {{ DF b ≈ b' ∈ per_typ_elem pred_P Δ ↘ R' }} ->
+    {{ SubT a' <: b' ∈ per_subtyp pred_P Δ }}.
+Proof.
+  mauto using per_subtyp_refl1, per_subtyp_refl2.
+Qed.
+
+#[export]
+Hint Resolve per_subtyp_transp : mcpts.
+ 
+(* Lemma per_subtyp_sorted_cumu {P} {pred_P : PredicativeSig P} : forall a1 a2 s, *)
+(*     {{ ⟪ pred_P ⟫ Subs a1 <: a2 at s }} -> *)
+(*     forall s', *)
+(*       st_subtyp s s' -> *)
+(*       {{ ⟪ pred_P ⟫ Subs a1 <: a2 at s' }}. *)
+(* Proof. *)
+(*   induction 1; intros; econstructor; mauto; *)
+(*     match_by_head (@per_sort P) ltac:(fun H => destruct H); *)
+(*     only 4: (etransitivity; eassumption); *)
+(*     eexists; mauto 2. *)
+(* Qed. *)
+
+(* #[export] *)
+(* Hint Resolve per_subtyp_sorted_cumu : mcpts. *)
+
+
+      
 (** Lemmas for per_gctx *)
 Lemma per_gctx_preserves_fresh {P} {pred_P : PredicativeSig P} : forall Δ Δ' x,
     {{ GC Δ ≈ Δ' ∈ per_gctx pred_P }} ->
@@ -1179,39 +1262,48 @@ Proof.
 Qed.
 
 #[export]
-Hint Resolve per_gctx_preserves_fresh. 
+Hint Resolve per_gctx_preserves_fresh : mcpts. 
 
 Lemma per_gctx_sym {P} {pred_P : PredicativeSig P} : forall Δ Δ',
     {{ GC Δ ≈ Δ' ∈ per_gctx pred_P }} ->
     {{ GC Δ' ≈ Δ ∈ per_gctx pred_P }}.
 Proof.
   induction 1; mauto 2.
-  symmetry in H2.
-  econstructor; mauto 2.
+  destruct_rel_typ_unsorted.
+  symmetry in H3.
+  symmetry in H6.
+  econstructor; mauto 2;
+    econstructor; mauto 2.
 Qed.
 
-Lemma per_gctx_trans {P} {pred_P : PredicativeSig P} : forall Δ Δ' Δ'',
-    {{ GC Δ ≈ Δ' ∈ per_gctx pred_P }} ->
-    {{ GC Δ' ≈ Δ'' ∈ per_gctx pred_P }} ->
-    {{ GC Δ ≈ Δ'' ∈ per_gctx pred_P }}.
-  intros * HΔΔ'.
-  gen Δ''.
-  induction HΔΔ'; intros * HΔ'Δ'';
-    dependent destruction HΔ'Δ'';
-    mauto 2.
+  
+(* Lemma per_gctx_trans {P} {pred_P : PredicativeSig P} : forall Δ Δ', *)
+(*     {{ GC Δ ≈ Δ' ∈ per_gctx pred_P }} -> *)
+(*     forall Δ'', *)
+(*       {{ GC Δ' ≈ Δ'' ∈ per_gctx pred_P }} -> *)
+(*       {{ GC Δ ≈ Δ'' ∈ per_gctx pred_P }}. *)
+(* Proof. *)
+(*   intros * HΔΔ'. *)
+(*   induction HΔΔ'; intros * HΔ'Δ''; *)
+(*     dependent destruction HΔ'Δ''; *)
+(*     mauto 2. *)
 
-  simplify_evals.
-  econstructor; mauto 3.
-  transitivity a'; mauto 2.
-Qed.
+(*   destruct_rel_typ_unsorted. *)
+(*   simplify_evals. *)
+(*   econstructor; mauto 3. *)
+(*   - econstructor; mauto 3. *)
+(*     etransitivity; mauto 2. *)
+(*     admit. *)
+(*   - transitivity a'; mauto 2. *)
+(* Qed. *)
 
-#[export]
-Instance per_gctx_PER {P} {pred_P : PredicativeSig P} : PER (per_gctx pred_P). 
-Proof.
-  split.
-  - mauto 3 using per_gctx_sym.
-  - mauto 3 using per_gctx_trans.
-Qed.
+(* #[export] *)
+(* Instance per_gctx_PER {P} {pred_P : PredicativeSig P} : PER (per_gctx pred_P).  *)
+(* Proof. *)
+(*   split. *)
+(*   - mauto 3 using per_gctx_sym. *)
+(*   - mauto 3 using per_gctx_trans. *)
+(* Qed. *)
 
 
 (** Lemmas for per_ctx_env and per_ctx *)
@@ -1234,7 +1326,7 @@ Proof.
 Qed.
 
 Lemma per_ctx_env_implies_per_gctx {P} {pred_P : PredicativeSig P} : forall Δ Γ Γ' R,
-    {{ EF Δ ; Γ ≈ Γ' ∈ per_ctx_env pred_P ↘ R }} ->
+    {{ EF Γ ≈ Γ' ∈ per_ctx_env pred_P Δ ↘ R }} ->
     {{ GC Δ ≈ Δ ∈ per_gctx pred_P }}.
 Proof.
   induction 1; mauto 2.
@@ -1246,10 +1338,10 @@ Hint Resolve per_ctx_env_implies_per_gctx : mcpts.
   
   
 Lemma per_ctx_env_right_irrel {P : PtsSig} {pred_P : PredicativeSig P} : forall Δ Γ Γ' Γ'' R R',
-    {{ EF Δ ; Γ ≈ Γ' ∈ per_ctx_env pred_P ↘ R }} ->
-    {{ EF Δ ; Γ ≈ Γ'' ∈ per_ctx_env pred_P ↘ R' }} ->
+    {{ EF Γ ≈ Γ' ∈ per_ctx_env pred_P Δ ↘ R }} ->
+    {{ EF Γ ≈ Γ'' ∈ per_ctx_env pred_P Δ ↘ R' }} ->
     R <~> R'.
-Proof with (destruct_rel_typ; handle_per_sort_elem_irrel; eexists; intuition).
+Proof with (destruct_rel_typ_unsorted; handle_per_typ_elem_irrel; eexists; intuition).
   intros * Horig; gen Γ'' R'.  
   induction Horig; intros * Hright;
     dependent destruction Hright; subst;
@@ -1260,8 +1352,8 @@ Proof with (destruct_rel_typ; handle_per_sort_elem_irrel; eexists; intuition).
     split; intros Hcons; dependent destruction Hcons;
     [ assert {{ Dom ρ ↯ ≈ ρ' ↯ ∈ tail_rel0 }} by intuition
     | assert {{ Dom ρ ↯ ≈ ρ' ↯ ∈ tail_rel }} by intuition ];
-    assert (rel_typ_unsorted pred_P A _ _ A' _ _ (head_rel _ _ ltac:(eassumption))) by mauto 3;
-    assert (rel_typ_unsorted pred_P A _ _ A'0 _ _ (head_rel0 _ _ ltac:(eassumption))) by mauto 3;
+    assert (rel_typ_unsorted pred_P _ A _ A' _ (head_rel _ _ ltac:(eassumption))) by mauto 3;
+    assert (rel_typ_unsorted pred_P _ A _ A'0 _ (head_rel0 _ _ ltac:(eassumption))) by mauto 3;
     inversion_clear_by_head (@rel_typ_unsorted P);
     simplify_evals;
     handle_per_typ_elem_irrel;
@@ -1269,35 +1361,11 @@ Proof with (destruct_rel_typ; handle_per_sort_elem_irrel; eexists; intuition).
     intuition.
 Qed.
 
-
-(* Lemma per_ctx_env_stable_under_per_gctx {P} {pred_P : PredicativeSig P} : forall Δ Γ Γ' R, *)
-(*     {{ EF Δ ; Γ ≈ Γ' ∈ per_ctx_env pred_P ↘ R }} -> *)
-(*     forall Δ', {{ GC Δ ≈ Δ' ∈ per_gctx pred_P }} -> *)
-(*           exists R', {{ EF Δ' ; Γ ≈ Γ' ∈ per_ctx_env pred_P ↘ R' }}. *)
-(* Proof. *)
-(*   induction 1; intros; *)
-(*     assert {{ GC Δ' ≈ Δ' ∈ per_gctx pred_P }} by (transitivity Δ; try eassumption; symmetry; eassumption); *)
-(*     mauto 3. *)
-
-(*   pose proof (IHper_ctx_env _ H2) as [tail_rel']. *)
-
-  
-(* Lemma per_ctx_env_up_to_per_gctx_irrel {P} {pred_P : PredicativeSig P} : forall Δ Δ' Γ Γ' R R', *)
-(*     {{ GC Δ ≈ Δ' ∈ per_gctx pred_P }} -> *)
-(*     {{ EF Δ ; Γ ≈ Γ' ∈ per_ctx_env pred_P ↘ R }} -> *)
-(*     {{ EF Δ' ; Γ ≈ Γ' ∈ per_ctx_env pred_P ↘ R' }} -> *)
-(*     R <~> R'. *)
-(* Proof. *)
-(*   intros * HΔΔ'; gen R' R Γ' Γ. *)
-(*   induction HΔΔ'. *)
-
-(*   - intros; mauto 2 using per_ctx_env_right_irrel. *)
-(*   - intros. *)
     
 
 Lemma per_ctx_env_sym {P : PtsSig} {pred_P : PredicativeSig P} : forall Δ Γ Γ' R,
-    {{ EF Δ ; Γ ≈ Γ' ∈ per_ctx_env pred_P ↘ R }} ->
-    {{ EF Δ ; Γ' ≈ Γ ∈ per_ctx_env pred_P ↘ R }} /\
+    {{ EF Γ ≈ Γ' ∈ per_ctx_env pred_P Δ ↘ R }} ->
+    {{ EF Γ' ≈ Γ ∈ per_ctx_env pred_P Δ ↘ R }} /\
       (forall ρ ρ',
           {{ Dom ρ ≈ ρ' ∈ R }} ->
           {{ Dom ρ' ≈ ρ ∈ R }}).
@@ -1323,15 +1391,15 @@ Proof with solve [intuition].
 Qed.
 
 Corollary per_ctx_sym {P : PtsSig} {pred_P : PredicativeSig P} : forall Δ Γ Γ' R,
-    {{ EF Δ ; Γ ≈ Γ' ∈ per_ctx_env pred_P ↘ R }} ->
-    {{ EF Δ ; Γ' ≈ Γ ∈ per_ctx_env pred_P ↘ R }}.
+    {{ EF Γ ≈ Γ' ∈ per_ctx_env pred_P Δ ↘ R }} ->
+    {{ EF Γ' ≈ Γ ∈ per_ctx_env pred_P Δ ↘ R }}.
 Proof.
   intros * ?%per_ctx_env_sym.
   firstorder.
 Qed.
 
 Corollary per_env_sym {P : PtsSig} {pred_P : PredicativeSig P} : forall Δ Γ Γ' R ρ ρ',
-    {{ EF Δ ; Γ ≈ Γ' ∈ per_ctx_env pred_P ↘ R }} ->
+    {{ EF Γ ≈ Γ' ∈ per_ctx_env pred_P Δ ↘ R }} ->
     {{ Dom ρ ≈ ρ' ∈ R }} ->
     {{ Dom ρ' ≈ ρ ∈ R }}.
 Proof.
@@ -1340,8 +1408,8 @@ Proof.
 Qed.
 
 Corollary per_ctx_env_left_irrel {P : PtsSig} {pred_P : PredicativeSig P} : forall Δ Γ Γ' Γ'' R R',
-    {{ EF Δ ; Γ ≈ Γ'' ∈ per_ctx_env pred_P ↘ R }} ->
-    {{ EF Δ ; Γ' ≈ Γ'' ∈ per_ctx_env pred_P ↘ R' }} ->
+    {{ EF Γ ≈ Γ'' ∈ per_ctx_env pred_P Δ ↘ R }} ->
+    {{ EF Γ' ≈ Γ'' ∈ per_ctx_env pred_P Δ ↘ R' }} ->
     R <~> R'.
 Proof.
   intros * ?%per_ctx_sym ?%per_ctx_sym.
@@ -1349,8 +1417,8 @@ Proof.
 Qed.
 
 Corollary per_ctx_env_cross_irrel {P : PtsSig} {pred_P : PredicativeSig P} : forall Δ Γ Γ' Γ'' R R',
-    {{ EF Δ ; Γ ≈ Γ' ∈ per_ctx_env pred_P ↘ R }} ->
-    {{ EF Δ ; Γ'' ≈ Γ ∈ per_ctx_env pred_P ↘ R' }} ->
+    {{ EF Γ ≈ Γ' ∈ per_ctx_env pred_P Δ ↘ R }} ->
+    {{ EF Γ'' ≈ Γ ∈ per_ctx_env pred_P Δ ↘ R' }} ->
     R <~> R'.
 Proof.
   intros * ? ?%per_ctx_sym.
@@ -1360,24 +1428,24 @@ Qed.
 Ltac do_per_ctx_env_irrel_assert1 :=
   let tactic_error o1 o2 := fail 3 "per_ctx_env_irrel equality between" o1 "and" o2 "cannot be solved" in
   match goal with
-    | H1 : {{ EF ^?Δ ; ^?Γ ≈ ^_ ∈ per_ctx_env ?pred_P ↘ ?R1 }},
-        H2 : {{ EF ^?Δ ; ^?Γ ≈ ^_ ∈ per_ctx_env ?pred_P ↘ ?R2 }} |- _ =>
+    | H1 : {{ EF ^?Γ ≈ ^_ ∈ per_ctx_env ?pred_P ?Δ ↘ ?R1 }},
+        H2 : {{ EF ^?Γ ≈ ^_ ∈ per_ctx_env ?pred_P ?Δ ↘ ?R2 }} |- _ =>
         assert_fails (unify R1 R2);
         match goal with
         | H : R1 <~> R2 |- _ => fail 1
         | H : R2 <~> R1 |- _ => fail 1
         | _ => assert (R1 <~> R2) by (eapply per_ctx_env_right_irrel; [apply H1 | apply H2]) || tactic_error R1 R2
         end
-    | H1 : {{ EF ^?Δ ; ^_ ≈ ^?Δ ∈ per_ctx_env ?pred_P ↘ ?R1 }},
-        H2 : {{ EF ^?Δ ; ^_ ≈ ^?Δ ∈ per_ctx_env ?pred_P ↘ ?R2 }} |- _ =>
+    | H1 : {{ EF ^_ ≈ ^?Δ ∈ per_ctx_env ?pred_P ?Δ ↘ ?R1 }},
+        H2 : {{ EF ^_ ≈ ^?Δ ∈ per_ctx_env ?pred_P ?Δ ↘ ?R2 }} |- _ =>
         assert_fails (unify R1 R2);
         match goal with
         | H : R1 <~> R2 |- _ => fail 1
         | H : R2 <~> R1 |- _ => fail 1
         | _ => assert (R1 <~> R2) by (eapply per_ctx_env_left_irrel; [apply H1 | apply H2]) || tactic_error R1 R2
         end
-    | H1 : {{ DF ^?Γ ≈ ^_ ∈ per_ctx_env ?pred_P ↘ ?R1 }},
-        H2 : {{ DF ^_ ≈ ^?Γ ∈ per_ctx_env ?pred_P ↘ ?R2 }} |- _ =>
+    | H1 : {{ DF ^?Γ ≈ ^_ ∈ per_ctx_env ?pred_P ?Δ ↘ ?R1 }},
+        H2 : {{ DF ^_ ≈ ^?Γ ∈ per_ctx_env ?pred_P ?Δ ↘ ?R2 }} |- _ =>
         (** Order matters less here as H1 and H2 cannot be exchanged *)
         assert_fails (unify R1 R2);
         match goal with
@@ -1396,16 +1464,16 @@ Ltac handle_per_ctx_env_irrel :=
   apply_relation_equivalence;
   clear_dups.
 
-Lemma per_ctx_env_trans {P : PtsSig} {pred_P : PredicativeSig P} : forall Γ1 Γ2 R,
-    {{ DF Γ1 ≈ Γ2 ∈ per_ctx_env pred_P ↘ R }} ->
+Lemma per_ctx_env_trans {P : PtsSig} {pred_P : PredicativeSig P} : forall Δ Γ1 Γ2 R,
+    {{ DF Γ1 ≈ Γ2 ∈ per_ctx_env pred_P Δ ↘ R }} ->
     (forall Γ3,
-        {{ DF Γ2 ≈ Γ3 ∈ per_ctx_env pred_P ↘ R }} ->
-        {{ DF Γ1 ≈ Γ3 ∈ per_ctx_env pred_P ↘ R }}) /\
+        {{ DF Γ2 ≈ Γ3 ∈ per_ctx_env pred_P Δ ↘ R }} ->
+        {{ DF Γ1 ≈ Γ3 ∈ per_ctx_env pred_P Δ ↘ R }}) /\
       (forall ρ1 ρ2 ρ3,
           {{ Dom ρ1 ≈ ρ2 ∈ R }} ->
           {{ Dom ρ2 ≈ ρ3 ∈ R }} ->
           {{ Dom ρ1 ≈ ρ3 ∈ R }}).
-Proof with solve [eauto using per_sort_trans].
+Proof with solve [eauto using per_typ_trans].
   simpl.
   induction 1; subst;
     [> split;
@@ -1433,17 +1501,17 @@ Proof with solve [eauto using per_sort_trans].
     eapply per_typ_elem_trans; intuition.
 Qed.
 
-Corollary per_ctx_trans {P : PtsSig} {pred_P : PredicativeSig P} : forall Γ1 Γ2 Γ3 R,
-    {{ DF Γ1 ≈ Γ2 ∈ per_ctx_env pred_P ↘ R }} ->
-    {{ DF Γ2 ≈ Γ3 ∈ per_ctx_env pred_P ↘ R }} ->
-    {{ DF Γ1 ≈ Γ3 ∈ per_ctx_env pred_P ↘ R }}.
+Corollary per_ctx_trans {P : PtsSig} {pred_P : PredicativeSig P} : forall Δ Γ1 Γ2 Γ3 R,
+    {{ DF Γ1 ≈ Γ2 ∈ per_ctx_env pred_P Δ ↘ R }} ->
+    {{ DF Γ2 ≈ Γ3 ∈ per_ctx_env pred_P Δ ↘ R }} ->
+    {{ DF Γ1 ≈ Γ3 ∈ per_ctx_env pred_P Δ ↘ R }}.
 Proof.
   intros * ?% per_ctx_env_trans.
   firstorder.
 Qed.
 
-Corollary per_env_trans {P : PtsSig} {pred_P : PredicativeSig P} : forall Γ1 Γ2 R ρ1 ρ2 ρ3,
-    {{ DF Γ1 ≈ Γ2 ∈ per_ctx_env pred_P ↘ R }} ->
+Corollary per_env_trans {P : PtsSig} {pred_P : PredicativeSig P} : forall Δ Γ1 Γ2 R ρ1 ρ2 ρ3,
+    {{ DF Γ1 ≈ Γ2 ∈ per_ctx_env pred_P Δ ↘ R }} ->
     {{ Dom ρ1 ≈ ρ2 ∈ R }} ->
     {{ Dom ρ2 ≈ ρ3 ∈ R }} ->
     {{ Dom ρ1 ≈ ρ3 ∈ R }}.
@@ -1453,7 +1521,7 @@ Proof.
 Qed.
 
 #[export]
-Instance per_ctx_PER {P : PtsSig} {pred_P : PredicativeSig P} {R} : PER (per_ctx_env pred_P R).
+Instance per_ctx_PER {P : PtsSig} {pred_P : PredicativeSig P} {Δ R} : PER (per_ctx_env pred_P Δ R).
 Proof.
   split.
   - auto using per_ctx_sym.
@@ -1461,22 +1529,22 @@ Proof.
 Qed.
 
 #[export]
-Instance per_env_PER {P : PtsSig} {pred_P : PredicativeSig P} {R Γ Δ} (H : per_ctx_env pred_P R Γ Δ) : PER R.
+Instance per_env_PER {P : PtsSig} {pred_P : PredicativeSig P} {Δ R Γ Γ'} (H : per_ctx_env pred_P Δ R Γ Γ') : PER R.
 Proof.
   split.
-  - pose proof (fun ρ ρ' => per_env_sym _ _ _ ρ ρ' H); auto.
-  - pose proof (fun ρ0 ρ1 ρ2 => per_env_trans _ _ _ ρ0 ρ1 ρ2 H); eauto.
+  - pose proof (fun ρ ρ' => per_env_sym _ _ _ _ ρ ρ' H); auto.
+  - pose proof (fun ρ0 ρ1 ρ2 => per_env_trans _ _ _ _ ρ0 ρ1 ρ2 H); eauto.
 Qed.
 
 (** This lemma removes the PER argument *)
-Lemma per_ctx_env_cons' {P : PtsSig} {pred_P : PredicativeSig P} : forall {Γ Γ' A A' tail_rel}
+Lemma per_ctx_env_cons' {P : PtsSig} {pred_P : PredicativeSig P} : forall {Δ Γ Γ' A A' tail_rel}
                              (head_rel : forall {ρ ρ'} (equiv_ρ_ρ' : {{ Dom ρ ≈ ρ' ∈ tail_rel }}), relation (domain P))
                              env_rel,
-    {{ EF Γ ≈ Γ' ∈ per_ctx_env pred_P ↘ tail_rel }} ->
+    {{ EF Γ ≈ Γ' ∈ per_ctx_env pred_P Δ ↘ tail_rel }} ->
     (forall {ρ ρ'} (equiv_ρ_ρ' : {{ Dom ρ ≈ ρ' ∈ tail_rel }}),
-        rel_typ_unsorted pred_P A ρ A' ρ' (head_rel equiv_ρ_ρ')) ->
+        rel_typ_unsorted pred_P Δ A ρ A' ρ' (head_rel equiv_ρ_ρ')) ->
     (env_rel <~> cons_per_ctx_env tail_rel (@head_rel)) ->
-    {{ EF Γ, A ≈ Γ', A' ∈ per_ctx_env pred_P ↘ env_rel }}.
+    {{ EF Γ, A ≈ Γ', A' ∈ per_ctx_env pred_P Δ ↘ env_rel }}.
 Proof.
   intros.
   econstructor; eauto.
@@ -1489,12 +1557,12 @@ Hint Resolve per_ctx_env_cons' : mcpts.
 Ltac per_ctx_env_econstructor :=
   (repeat intro; hnf; eapply per_ctx_env_cons') + econstructor.
 
-Lemma per_ctx_env_cons_clean_inversion {P : PtsSig} {pred_P : PredicativeSig P} : forall {Γ Γ' env_relΓ A A' env_relΓA},
-    {{ EF Γ ≈ Γ' ∈ per_ctx_env pred_P ↘ env_relΓ }} ->
-    {{ EF Γ, A ≈ Γ', A' ∈ per_ctx_env pred_P ↘ env_relΓA }} ->
+Lemma per_ctx_env_cons_clean_inversion {P : PtsSig} {pred_P : PredicativeSig P} : forall {Δ Γ Γ' env_relΓ A A' env_relΓA},
+    {{ EF Γ ≈ Γ' ∈ per_ctx_env pred_P Δ ↘ env_relΓ }} ->
+    {{ EF Γ, A ≈ Γ', A' ∈ per_ctx_env pred_P Δ ↘ env_relΓA }} ->
     exists (head_rel : forall {ρ ρ'} (equiv_ρ_ρ' : {{ Dom ρ ≈ ρ' ∈ env_relΓ }}), relation (domain P)),
       (forall ρ ρ' (equiv_ρ_ρ' : {{ Dom ρ ≈ ρ' ∈ env_relΓ }}),
-          rel_typ_unsorted pred_P A ρ A' ρ' (head_rel equiv_ρ_ρ')) /\
+          rel_typ_unsorted pred_P Δ A ρ A' ρ' (head_rel equiv_ρ_ρ')) /\
         (env_relΓA <~> cons_per_ctx_env env_relΓ (@head_rel)).
 Proof with intuition.
   intros * HΓ HΓA.
@@ -1504,7 +1572,7 @@ Proof with intuition.
   split; intros.
   - instantiate (1 := fun ρ ρ' (equiv_ρ_ρ' : env_relΓ ρ ρ') m m' =>
                         forall R,
-                          rel_typ_unsorted pred_P A ρ A' ρ' R ->
+                          rel_typ_unsorted pred_P Δ A ρ A' ρ' R ->
                           {{ Dom m ≈ m' ∈ R }}).
     assert (tail_rel ρ ρ') by intuition.
     (on_all_hyp: destruct_rel_by_assumption tail_rel).
@@ -1530,26 +1598,39 @@ Ltac invert_per_ctx_envs := match_by_head per_ctx_env ltac:(fun H => directed in
 
 Ltac invert_per_ctx_envs_of pred_P rel := match_by_head (per_ctx_env pred_P rel) ltac:(fun H => directed invert_per_ctx_env H).
 
-Lemma per_ctx_respects_length {P : PtsSig} {pred_P : PredicativeSig P} : forall {Γ Γ'},
-    {{ Exp Γ ≈ Γ' ∈ per_ctx pred_P }} ->
+Lemma per_ctx_respects_length {P : PtsSig} {pred_P : PredicativeSig P} : forall {Δ Γ Γ'},
+    {{ GC Γ ≈ Γ' ∈ per_ctx pred_P Δ }} ->
     length Γ = length Γ'.
 Proof.
   intros * [? H].
   induction H; simpl; congruence.
 Qed.
 
-Lemma per_ctx_subtyp_to_env {P : PtsSig} {pred_P : PredicativeSig P} : forall Γ Δ,
-    {{ ⟪ pred_P ⟫ SubE Γ <: Δ }} ->
-    exists R R',
-      {{ EF Γ ≈ Γ ∈ per_ctx_env pred_P ↘ R }} /\
-        {{ EF Δ ≈ Δ ∈ per_ctx_env pred_P ↘ R' }}.
+
+Lemma per_ctx_subtyp_implies_per_gctx {P} {pred_P : PredicativeSig P} : forall Δ Γ Γ',
+    {{ SubC Γ <: Γ' ∈ per_ctx_subtyp pred_P Δ }} ->
+    {{ GC Δ ≈ Δ ∈ per_gctx pred_P }}.
 Proof.
-  destruct 1; destruct_all.
-  - repeat eexists; econstructor; apply Equivalence_Reflexive.
+  induction 1; mauto 2.
+Qed.
+
+#[export]
+Hint Resolve per_ctx_subtyp_implies_per_gctx : mcpts.
+
+Lemma per_ctx_subtyp_to_env {P : PtsSig} {pred_P : PredicativeSig P} : forall Δ Γ Γ',
+    {{ SubC Γ <: Γ' ∈ per_ctx_subtyp pred_P Δ }} ->
+    exists R R',
+      {{ EF Γ ≈ Γ ∈ per_ctx_env pred_P Δ ↘ R }} /\
+        {{ EF Γ' ≈ Γ' ∈ per_ctx_env pred_P Δ ↘ R' }}.
+Proof.
+  intros * HΓΓ'.
+  assert {{ GC Δ ≈ Δ ∈ per_gctx pred_P }} by mauto 2.
+  destruct HΓΓ'; destruct_all.
+  - repeat eexists; econstructor; try apply Equivalence_Reflexive; try eassumption.
   - eauto.
 Qed.
 
-Add Parametric Morphism {P} {pred_P : PredicativeSig P} A ρ A' ρ' : (rel_typ_unsorted pred_P A ρ A' ρ')
+Add Parametric Morphism {P} {pred_P : PredicativeSig P} Δ A ρ A' ρ' : (rel_typ_unsorted pred_P Δ A ρ A' ρ')
     with signature (@relation_equivalence (domain P)) ==> iff as rel_typ_unsorted_morphism.
 Proof.
   intros * HRR'.
@@ -1557,31 +1638,31 @@ Proof.
     [setoid_rewrite <- HRR' | setoid_rewrite HRR']; eassumption.
 Qed.
 
-Lemma rel_typ_implies_rel_typ_unsorted {P} {pred_P : PredicativeSig P} : forall s A ρ A' ρ' R,
-    rel_typ pred_P s A ρ A' ρ' R ->
-    rel_typ_unsorted pred_P A ρ A' ρ' R.
-Proof.
-  intros * Hsorted.
-  destruct Hsorted.
-  econstructor; mauto.
-Qed.
+(* Lemma rel_typ_implies_rel_typ_unsorted {P} {pred_P : PredicativeSig P} : forall s A ρ A' ρ' R, *)
+(*     rel_typ pred_P s A ρ A' ρ' R -> *)
+(*     rel_typ_unsorted pred_P A ρ A' ρ' R. *)
+(* Proof. *)
+(*   intros * Hsorted. *)
+(*   destruct Hsorted. *)
+(*   econstructor; mauto. *)
+(* Qed. *)
 
-#[export]
-Hint Resolve rel_typ_implies_rel_typ_unsorted : mcpts.
+(* #[export] *)
+(* Hint Resolve rel_typ_implies_rel_typ_unsorted : mcpts. *)
 
 
-Lemma per_ctx_env_cons_clean_inversion_unsorted {P : PtsSig} (pred_P : PredicativeSig P) : forall {Γ Γ' env_relΓ A A' env_relΓA},
-    {{ EF Γ ≈ Γ' ∈ per_ctx_env pred_P ↘ env_relΓ }} ->
-    {{ EF Γ, A ≈ Γ', A' ∈ per_ctx_env pred_P ↘ env_relΓA }} ->
+Lemma per_ctx_env_cons_clean_inversion_unsorted {P : PtsSig} (pred_P : PredicativeSig P) : forall {Δ Γ Γ' env_relΓ A A' env_relΓA},
+    {{ EF Γ ≈ Γ' ∈ per_ctx_env pred_P Δ ↘ env_relΓ }} ->
+    {{ EF Γ, A ≈ Γ', A' ∈ per_ctx_env pred_P Δ ↘ env_relΓA }} ->
     exists (head_rel : forall {ρ ρ'} (equiv_ρ_ρ' : {{ Dom ρ ≈ ρ' ∈ env_relΓ }}), relation (domain P)),
       (forall ρ ρ' (equiv_ρ_ρ' : {{ Dom ρ ≈ ρ' ∈ env_relΓ }}),
-          rel_typ_unsorted pred_P A ρ A' ρ' (head_rel equiv_ρ_ρ')) /\
+          rel_typ_unsorted pred_P Δ A ρ A' ρ' (head_rel equiv_ρ_ρ')) /\
         (env_relΓA <~> cons_per_ctx_env env_relΓ (@head_rel)).
 Proof with intuition.
   intros * HΓ HΓA.
   assert (exists (head_rel : forall {ρ ρ'} (equiv_ρ_ρ' : {{ Dom ρ ≈ ρ' ∈ env_relΓ }}), relation (domain P)),
       (forall ρ ρ' (equiv_ρ_ρ' : {{ Dom ρ ≈ ρ' ∈ env_relΓ }}),
-          rel_typ_unsorted pred_P A ρ A' ρ' (head_rel equiv_ρ_ρ')) /\
+          rel_typ_unsorted pred_P Δ A ρ A' ρ' (head_rel equiv_ρ_ρ')) /\
         (env_relΓA <~> cons_per_ctx_env env_relΓ (@head_rel))) by (eapply per_ctx_env_cons_clean_inversion; mauto).
   destruct_conjs.
   eexists.
@@ -1595,200 +1676,12 @@ Ltac invert_per_ctx_env_unsorted H :=
 Ltac invert_per_ctx_envs_unsorted := match_by_head per_ctx_env ltac:(fun H => directed invert_per_ctx_env_unsorted H).
 Ltac invert_per_ctx_envs_unsorted_of pred_P rel := match_by_head (per_ctx_env pred_P rel) ltac:(fun H => directed invert_per_ctx_env_unsorted H).
 
-Lemma per_typ_elem_and_per_sort_elem_implies_per_sort_elem {P} (pred_P : PredicativeSig P) : forall { a b c R R' s},
-    {{ DF a ≈ b ∈ per_typ_elem pred_P ↘ R }} ->
-    {{ DF a ≈ c ∈ per_sort_elem pred_P s ↘ R' }} ->
-    {{ DF a ≈ b ∈ per_sort_elem pred_P s ↘ R }}.
-Proof.
-  intros * Hab.
-  inversion_clear Hab; intros.
-  - invert_per_sort_elem H0; mauto.
-  - handle_per_sort_elem_irrel.
-    assert (per_sort_elem pred_P s R c a) by (eapply (per_sort_elem_sym H0); mauto).
-    assert (per_sort_elem pred_P s R c b) by (eapply (per_sort_elem_trans s R c a H1); eassumption).
-    eapply (per_sort_elem_trans s R a c H0); eassumption.
-Qed.
 
-#[export]
-Hint Resolve per_typ_elem_and_per_sort_elem_implies_per_sort_elem : mcpts.
-
-
-
-Lemma per_subtyp_to_typ_elem {P} {pred_P : PredicativeSig P} : forall a b,
-    {{ ⟪ pred_P ⟫ Sub a <: b }} ->
-    exists R R',
-      {{ DF a ≈ a ∈ per_typ_elem pred_P ↘ R }} /\
-        {{ DF b ≈ b ∈ per_typ_elem pred_P ↘ R' }}.
-Proof.
-  destruct 1.
-  - repeat eexists; econstructor; reflexivity.
-  - pose proof (per_subtyp_sorted_to_sort_elem a b s H).
-    destruct_conjs.
-    repeat eexists; econstructor; eassumption.
-Qed.
-
-
-Lemma per_elem_subtyping {P} {pred_P : PredicativeSig P} : forall A B,
-    {{ ⟪ pred_P ⟫ Sub A <: B }} ->
-    forall R R' a b,
-      {{ DF A ≈ A ∈ per_typ_elem pred_P ↘ R }} ->
-      {{ DF B ≈ B ∈ per_typ_elem pred_P ↘ R' }} ->
-      R a b ->
-      R' a b.
-Proof.
-  destruct 1.
-  - intros.
-    assert (per_typ_elem pred_P (per_sort pred_P s1) d{{{ Sort@s1 }}} d{{{ Sort@s1 }}}) by (econstructor; reflexivity).
-    assert (per_typ_elem pred_P (per_sort pred_P s2) d{{{ Sort@s2 }}} d{{{ Sort@s2 }}}) by (econstructor; reflexivity).
-    handle_per_typ_elem_irrel.
-    destruct H2 as [R].
-    eexists; mauto 2.
-  - intros.
-    pose proof (per_subtyp_sorted_to_sort_elem a b s H).
-    destruct_conjs.
-    assert (per_typ_elem pred_P H3 a a) by mauto 2.
-    assert (per_typ_elem pred_P H4 b b) by mauto 2.
-    handle_per_typ_elem_irrel.
-    eapply per_elem_subtyping_sorted; mauto 2.
-Qed.    
-
-
-Lemma per_elem_subtyping_gen {P} {pred_P : PredicativeSig P} : forall a b a' b' R R' m n,
-    {{ ⟪ pred_P ⟫ Sub a <: b }} ->
-    {{ DF a ≈ a' ∈ per_typ_elem pred_P ↘ R }} ->
-    {{ DF b ≈ b' ∈ per_typ_elem pred_P ↘ R' }} ->
-    R m n ->
-    R' m n.
-Proof.
-  intros.
-  eapply per_elem_subtyping; saturate_refl; try eassumption.
-Qed.
-
-Lemma per_subtyp_refl1 {P} {pred_P : PredicativeSig P} : forall a b R,
-    {{ DF a ≈ b ∈ per_typ_elem pred_P ↘ R }} ->
-    {{ ⟪ pred_P ⟫ Sub a <: b }}.
-Proof.
-  simpl; destruct 1.
-  - econstructor; mauto 2.
-  - pose proof (per_subtyp_sorted_refl1 _ _ _ _ H).
-    econstructor; mauto 2.
-Qed.
-
-#[export]
-Hint Resolve per_subtyp_refl1 : mcpts.
-
-Lemma per_subtyp_refl2 {P} {pred_P : PredicativeSig P} : forall a b R,
-    {{ DF a ≈ b ∈ per_typ_elem pred_P ↘ R }} ->
-    {{ ⟪ pred_P ⟫ Sub b <: a }}.
-Proof.
-  intros.
-  symmetry in H.
-  eauto using per_subtyp_refl1.
-Qed.
-
-#[export]
-Hint Resolve per_subtyp_refl2 : mcpts.
-
-    
-Lemma per_subtyp_trans_helper {P} {pred_P : PredicativeSig P} : forall {a1 a2 s},
-    {{ ⟪ pred_P ⟫ Subs a1 <: a2 at s }} ->
-    forall a3 s',
-      {{ ⟪ pred_P ⟫ Subs a2 <: a3 at s' }} ->
-      {{ ⟪ pred_P ⟫ Sub a1 <: a3 }}.
-Proof.
-  induction 1; intros ? ? Hsub; simpl in *.
-  - dependent destruction Hsub.
-    assert (st_subtyp s1 s3) by (transitivity s2; eauto).
-    econstructor; mauto 2.
-  - econstructor; mauto 2.
-  - dependent destruction Hsub.
-    handle_per_sort_elem_irrel.
-    assert (per_sort_elem pred_P s elem_rel'0 d{{{ Π r a'0 ρ'0 B'0 }}} d{{{ Π r a'0 ρ'0 B'0 }}}).
-    {
-      invert_per_sort_elem H7.
-      
-      per_sort_elem_econstructor; mauto 2.
-      - pose proof (ord_ru_pi_sub pred_P r sub1) as [ord_dom ord_im].
-        destruct_conjs.
-        destruct ord_dom; subst; mauto 2.
-      - intros.
-        destruct_rel_mod_eval.
-        pose proof (ord_ru_pi_sub pred_P r sub1) as [ord_dom ord_im].
-        destruct_conjs.
-        econstructor; mauto 2.
-        destruct ord_im; subst; mauto 2.
-    }
-    eapply per_subtyp_from_sorted with (s := s).
-    econstructor; mauto 2.
-    + transitivity a'; eauto.
-    + intros.      
-      invert_per_sort_elem H3.
-      assert (per_sort_elem pred_P s1 in_rel a' a').
-      {
-        pose proof (ord_ru_pi_sub pred_P r sub) as [ord_dom ord_im].
-        destruct_conjs.
-        destruct ord_dom; subst; mauto 2.
-      }
-      handle_per_sort_elem_irrel.
-      destruct_rel_mod_eval.
-      assert (per_sort_elem pred_P s2 (out_rel c c' H11) a0 a'1).
-      {
-        pose proof (ord_ru_pi_sub pred_P r sub0) as [ord_dom ord_im].
-        destruct_conjs.
-        destruct ord_im; subst; mauto 2.
-      }
-      assert (per_subtyp_sorted pred_P s2 a'1 a0) by mauto 3.
-      assert (per_subtyp_sorted pred_P s2 b a'1) by mauto 3.
-      assert (per_subtyp_sorted pred_P s2 a0 b') by mauto 3.
-      transitivity a'1; eauto.
-      transitivity a0; eauto.
-  - econstructor; mauto 3.
-Qed.
-
-Lemma per_subtyp_trans {P} {pred_P : PredicativeSig P} : forall a1 a2,
-    {{ ⟪ pred_P ⟫ Sub a1 <: a2 }} ->
-    forall a3,
-      {{ ⟪ pred_P ⟫ Sub a2 <: a3 }} ->
-      {{ ⟪ pred_P ⟫ Sub a1 <: a3 }}.
-Proof.
-  destruct 1; intros ? Hsub; simpl in *; mauto 2.
-  - assert {{ ⟪ pred_P ⟫ Sub Sort@s1 <: Sort@s2 }} by mauto 2.
-    dependent destruction Hsub.
-    + econstructor; mauto 2.
-      transitivity s2; eauto.
-    + dependent destruction H0.
-      econstructor; mauto 2.
-      transitivity s2; eauto.
-  - destruct Hsub.
-    + dependent destruction H.
-      econstructor.
-      etransitivity; eauto.
-    + eapply per_subtyp_trans_helper; mauto 2.
-Qed.
-  
-#[export]
-Hint Resolve per_subtyp_trans : mcpts.
-
-#[export]
-Instance per_subtyp_trans_ins {P} {pred_P : PredicativeSig P} : Transitive (per_subtyp pred_P).
-Proof.
-  eauto using per_subtyp_trans.
-Qed.
-
-Lemma per_subtyp_transp {P} {pred_P : PredicativeSig P} : forall a b a' b' R R',
-    {{ ⟪ pred_P ⟫ Sub a <: b }} ->
-    {{ DF a ≈ a' ∈ per_typ_elem pred_P ↘ R }} ->
-    {{ DF b ≈ b' ∈ per_typ_elem pred_P ↘ R' }} ->
-    {{ ⟪ pred_P ⟫ Sub a' <: b' }}.
-Proof.
-  mauto using per_subtyp_refl1, per_subtyp_refl2.
-Qed.
-
-Lemma per_ctx_env_subtyping {P : PtsSig} {pred_P : PredicativeSig P} : forall Γ Δ,
-    {{ ⟪ pred_P ⟫ SubE Γ <: Δ }} ->
+Lemma per_ctx_env_subtyping {P : PtsSig} {pred_P : PredicativeSig P} : forall Δ Γ Γ',
+    {{ SubC Γ <: Γ' ∈ per_ctx_subtyp pred_P Δ }} ->
     forall R R' ρ ρ',
-      {{ EF Γ ≈ Γ ∈ per_ctx_env pred_P ↘ R }} ->
-      {{ EF Δ ≈ Δ ∈ per_ctx_env pred_P ↘ R' }} ->
+      {{ EF Γ ≈ Γ ∈ per_ctx_env pred_P Δ ↘ R }} ->
+      {{ EF Γ' ≈ Γ' ∈ per_ctx_env pred_P Δ ↘ R' }} ->
       R ρ ρ' ->
       R' ρ ρ'.
 Proof.
@@ -1804,20 +1697,20 @@ Proof.
    
   destruct_rel_typ_unsorted.
   eapply per_elem_subtyping; try eassumption.
-  - eauto using per_subtyp_sorted_cumu.
+  - eauto.
   - saturate_refl.
     mauto.
   - saturate_refl.
     mauto.
 Qed.
 
-Lemma per_ctx_subtyp_refl1 {P : PtsSig} {pred_P : PredicativeSig P} : forall Γ Δ R,
-    {{ EF Γ ≈ Δ ∈ per_ctx_env pred_P ↘ R }} ->
-    {{ ⟪ pred_P ⟫ SubE Γ <: Δ }}.
+Lemma per_ctx_subtyp_refl1 {P : PtsSig} {pred_P : PredicativeSig P} : forall Δ Γ Γ' R,
+    {{ EF Γ ≈ Γ' ∈ per_ctx_env pred_P Δ ↘ R }} ->
+    {{ SubC Γ <: Γ' ∈ per_ctx_subtyp pred_P Δ }}.
 Proof.
   induction 1; mauto.
 
-  assert (exists R, {{ EF Γ , A ≈ Γ' , A' ∈ per_ctx_env pred_P ↘ R }}) by
+  assert (exists R, {{ EF Γ , A ≈ Γ' , A' ∈ per_ctx_env pred_P Δ ↘ R }}) by
     (eexists; eapply per_ctx_env_cons'; eassumption).
   destruct_all.
   econstructor; try solve [saturate_refl; mauto 2].
@@ -1827,18 +1720,18 @@ Proof.
   mauto.
 Qed.
 
-Lemma per_ctx_subtyp_refl2 {P : PtsSig} {pred_P : PredicativeSig P} : forall Γ Δ R,
-    {{ EF Γ ≈ Δ ∈ per_ctx_env pred_P ↘ R }} ->
-    {{ ⟪ pred_P ⟫ SubE Δ <: Γ }}.
+Lemma per_ctx_subtyp_refl2 {P : PtsSig} {pred_P : PredicativeSig P} : forall Δ Γ Γ' R,
+    {{ EF Γ ≈ Γ' ∈ per_ctx_env pred_P Δ ↘ R }} ->
+    {{ SubC Γ' <: Γ ∈ per_ctx_subtyp pred_P Δ }}.
 Proof.
   intros. symmetry in H. eauto using per_ctx_subtyp_refl1.
 Qed.
 
-Lemma per_ctx_subtyp_trans {P : PtsSig} {pred_P : PredicativeSig P} : forall Γ1 Γ2,
-    {{ ⟪ pred_P ⟫ SubE Γ1 <: Γ2 }} ->
+Lemma per_ctx_subtyp_trans {P : PtsSig} {pred_P : PredicativeSig P} : forall Δ Γ1 Γ2,
+    {{ SubC Γ1 <: Γ2 ∈ per_ctx_subtyp pred_P Δ }} ->
     forall Γ3,
-      {{ ⟪ pred_P ⟫ SubE Γ2 <: Γ3 }} ->
-      {{ ⟪ pred_P ⟫ SubE Γ1 <: Γ3 }}.
+      {{ SubC Γ2 <: Γ3 ∈ per_ctx_subtyp pred_P Δ }} ->
+      {{ SubC Γ1 <: Γ3 ∈ per_ctx_subtyp pred_P Δ }}.
 Proof.
   induction 1; intros;
     dir_inversion_by_head (@per_ctx_subtyp P); subst;
@@ -1854,7 +1747,7 @@ Proof.
     saturate_refl_for tail_rel.
     destruct_rel_typ_unsorted.
     handle_per_typ_elem_irrel.
-    etransitivity; intuition mauto using per_subtyp_sorted_cumu.
+    etransitivity; intuition mauto.
   - econstructor; intuition.
     + typeclasses eauto.
     + solve_refl.
@@ -1867,111 +1760,98 @@ Qed.
 Hint Resolve per_ctx_subtyp_trans : mcpts.
 
 #[export]
-Instance per_ctx_subtyp_trans_ins {P : PtsSig} {pred_P : PredicativeSig P} : Transitive (@per_ctx_subtyp P pred_P).
+Instance per_ctx_subtyp_trans_ins {P : PtsSig} {pred_P : PredicativeSig P} {Δ} : Transitive (per_ctx_subtyp pred_P Δ).
 Proof.
   eauto using per_ctx_subtyp_trans.
 Qed.
 
 
-Lemma per_sort_elem_pi_lowering {P} (pred_P : PredicativeSig P) : forall {s1 s2 s3 s} {r : Ru_pi P s1 s2 s3} {elem_rel a ρ B a' ρ' B'},
-    {{ DF Π r a ρ B ≈ Π r a' ρ' B' ∈ per_sort_elem pred_P s ↘ elem_rel }} ->
-    {{ DF Π r a ρ B ≈ Π r a' ρ' B' ∈ per_sort_elem pred_P s3 ↘ elem_rel }}.
-Proof.
-  intros.
-  invert_per_sort_elem H.
-  per_sort_elem_econstructor; mauto 3.
-  - destruct_conjs.
-    pose proof ord_ru_pi_sub pred_P r sub as [[] ?]; subst; mauto 2.
-  - intros.
-    destruct_rel_mod_eval.
-    econstructor; mauto 3.
-    pose proof ord_ru_pi_sub pred_P r sub as [? []]; subst; mauto 2.
-Qed.
 
+(* Lemma per_subtyp_implies_per_subtyp_sorted {P} {pred_P : PredicativeSig P} : forall b b', *)
+(*     {{ ⟪ pred_P ⟫ Sub b <: b' }} -> *)
+(*     forall s s1 s2, *)
+(*       {{ Dom b ≈ b ∈ per_sort pred_P s1 }} -> *)
+(*       {{ Dom b' ≈ b' ∈ per_sort pred_P s2 }} -> *)
+(*       st_subtyp s1 s -> *)
+(*       st_subtyp s2 s -> *)
+(*       {{ ⟪ pred_P ⟫ Subs b <: b' at s }}. *)
+(* Proof. *)
+(*   intros * H. *)
+(*   destruct H. *)
+(*   - intros. *)
+(*     destruct_by_head @per_sort. *)
+(*     econstructor; mauto. *)
+(*   - induction H. *)
+(*     + intros. *)
+(*       destruct_by_head @per_sort. *)
+(*       handle_per_sort_elem_irrel. *)
+(*       econstructor; mauto. *)
+(*     + mauto. *)
+(*     + intros. *)
+(*       destruct_by_head @per_sort. *)
+(*       handle_per_sort_elem_irrel. *)
+(*       assert (per_sort_elem pred_P s0 elem_rel d{{{ Π r a ρ B }}} d{{{ Π r a ρ B }}}) by mauto. *)
+(*       invert_per_sort_elem H8. *)
+(*       econstructor; mauto. *)
+(*     + mauto. *)
+(* Qed. *)
 
-Lemma per_subtyp_implies_per_subtyp_sorted {P} {pred_P : PredicativeSig P} : forall b b',
-    {{ ⟪ pred_P ⟫ Sub b <: b' }} ->
-    forall s s1 s2,
-      {{ Dom b ≈ b ∈ per_sort pred_P s1 }} ->
-      {{ Dom b' ≈ b' ∈ per_sort pred_P s2 }} ->
-      st_subtyp s1 s ->
-      st_subtyp s2 s ->
-      {{ ⟪ pred_P ⟫ Subs b <: b' at s }}.
-Proof.
-  intros * H.
-  destruct H.
-  - intros.
-    destruct_by_head @per_sort.
-    econstructor; mauto.
-  - induction H.
-    + intros.
-      destruct_by_head @per_sort.
-      handle_per_sort_elem_irrel.
-      econstructor; mauto.
-    + mauto.
-    + intros.
-      destruct_by_head @per_sort.
-      handle_per_sort_elem_irrel.
-      assert (per_sort_elem pred_P s0 elem_rel d{{{ Π r a ρ B }}} d{{{ Π r a ρ B }}}) by mauto.
-      invert_per_sort_elem H8.
-      econstructor; mauto.
-    + mauto.
-Qed.
-
-Lemma per_subtyp_sort_inv_left {P} (pred_P : PredicativeSig P) : forall {s a},
-    {{ ⟪ pred_P ⟫ Sub Sort@s <: a }} ->
+Lemma per_subtyp_sort_inv_left {P} (pred_P : PredicativeSig P) : forall {Δ s a},
+    {{ SubT Sort@s <: a ∈ per_subtyp pred_P Δ }} ->
     exists s', a = d{{{ Sort@s' }}} /\ st_subtyp s s'.
 Proof.
+  simpl.
   intros.
   do 2 (dependent destruction H; mauto).
 Qed.
 
-Lemma per_subtyp_sort_inv_right {P} (pred_P : PredicativeSig P) : forall {s a},
-    {{ ⟪ pred_P ⟫ Sub a <: Sort@s }} ->
+Lemma per_subtyp_sort_inv_right {P} (pred_P : PredicativeSig P) : forall {Δ s a},
+    {{ SubT a <: Sort@s ∈ per_subtyp pred_P Δ }} ->
     exists s', a = d{{{ Sort@s' }}} /\ st_subtyp s' s.
 Proof.
+  simpl.
   intros.
   do 2 (dependent destruction H; mauto).
 Qed.
 
-Lemma per_subtyp_nat_inv_left {P} (pred_P : PredicativeSig P) : forall {a},
-    {{ ⟪ pred_P ⟫ Sub ℕ <: a }} ->
+Lemma per_subtyp_nat_inv_left {P} (pred_P : PredicativeSig P) : forall {Δ a},
+    {{ SubT ℕ <: a ∈ per_subtyp pred_P Δ }} ->
     (a = d{{{ ℕ }}}).
 Proof.
   intros.
   inversion_clear H.
-  inversion_clear H0.
   reflexivity.
 Qed.
 
-Lemma per_subtyp_nat_inv_right {P} (pred_P : PredicativeSig P) : forall {a},
-    {{ ⟪ pred_P ⟫ Sub a <: ℕ }} ->
+Lemma per_subtyp_nat_inv_right {P} (pred_P : PredicativeSig P) : forall {Δ a},
+    {{ SubT a <: ℕ ∈ per_subtyp pred_P Δ }} ->
     a = d{{{ ℕ }}}.
 Proof.
   intros.
   inversion_clear H.
-  inversion_clear H0.
   reflexivity.
 Qed.
 
-Lemma per_subtyp_pi_inv_left {P} (pred_P : PredicativeSig P) : forall {s1 s2 s3 c a ρ B} {r : Ru_pi P s1 s2 s3},
-    {{ ⟪ pred_P ⟫ Sub Π r a ρ B <: c }} ->
+Lemma per_subtyp_pi_inv_left {P} (pred_P : PredicativeSig P) : forall {Δ s1 s2 s3 c a ρ B} {r : Ru_pi P s1 s2 s3},
+    {{ SubT Π r a ρ B <: c ∈ per_subtyp pred_P Δ }} ->
     exists a' ρ' B', c = d{{{ Π r a' ρ' B' }}}.
 Proof.
+  simpl.
   intros.
   do 2 (dependent destruction H; mauto).
 Qed.
 
-Lemma per_subtyp_pi_inv_right {P} (pred_P : PredicativeSig P) : forall {s1 s2 s3 c a ρ B} {r : Ru_pi P s1 s2 s3},
-    {{ ⟪ pred_P ⟫ Sub c <: Π r a ρ B }} ->
+Lemma per_subtyp_pi_inv_right {P} (pred_P : PredicativeSig P) : forall {Δ s1 s2 s3 c a ρ B} {r : Ru_pi P s1 s2 s3},
+    {{ SubT c <: Π r a ρ B ∈ per_subtyp pred_P Δ }} ->
     exists a' ρ' B', c = d{{{ Π r a' ρ' B' }}}.
 Proof.
+  simpl.
   intros.
   do 2 (dependent destruction H; mauto).
 Qed.
 
-Lemma per_bot_var_inv {P : PtsSig} : forall {n n'},
-    @per_bot P d{{{ !n }}} d{{{ !n' }}} ->
+Lemma per_bot_var_inv {P : PtsSig} : forall {Δ : gctx P} {n n'},
+    per_bot Δ d{{{ !n }}} d{{{ !n' }}} ->
     n = n'.
 Proof.
   intros.
@@ -1981,36 +1861,70 @@ Proof.
   lia.
 Qed.
 
-Lemma per_subtyp_var_inv_left {P} (pred_P : PredicativeSig P) : forall {a x n l},
+Lemma per_subtyp_var_inv_left {P} (pred_P : PredicativeSig P) : forall {Δ a x n l},
     n < l ->
-    {{ ⟪ pred_P ⟫ Sub ⇑! x n <: a }} ->
+    {{ SubT ⇑! x n <: a ∈ per_subtyp pred_P Δ}} ->
     exists x', a = d{{{ ⇑! x' n }}}.
 Proof.
   intros * Hlt ?.
   inversion_clear H.
-  inversion_clear H0.
-  pose proof H.
-  specialize (H l) as [M []].
-  inversion H; subst.
+  pose proof H0.
+  specialize (H0 l) as [M []].
+  inversion H0; subst.
   inversion H1; subst.
+  assert (x0 = n) by (eapply per_bot_var_inv; mauto 2).
+  subst.
+  eexists; reflexivity.
+Qed.
+
+Lemma per_subtyp_var_inv_right {P} (pred_P : PredicativeSig P) : forall {Δ a x n l},
+    n < l ->
+    {{ SubT a <: ⇑! x n ∈ per_subtyp pred_P Δ }} ->
+    exists x', a = d{{{ ⇑! x' n }}}.
+Proof.
+  intros * Hlt ?.
+  inversion_clear H.
+  pose proof H0.
+  specialize (H0 l) as [M []].
+  inversion H1; subst.
+  inversion H0; subst.
   assert (n = x0) by (eapply per_bot_var_inv; mauto 2).
   subst.
   eexists; reflexivity.
 Qed.
 
-Lemma per_subtyp_var_inv_right {P} (pred_P : PredicativeSig P) : forall {a x n l},
-    n < l ->
-    {{ ⟪ pred_P ⟫ Sub a <: ⇑! x n }} ->
-    exists x', a = d{{{ ⇑! x' n }}}.
+
+Lemma per_bot_gvar_inv {P : PtsSig} : forall {Δ : gctx P} {x x'},
+    per_bot Δ d{{{ `!x }}} d{{{ `!x' }}} ->
+    x = x'.
 Proof.
-  intros * Hlt ?.
-  inversion_clear H.
-  inversion_clear H0.
-  pose proof H.
-  specialize (H l) as [M []].
-  inversion H1; subst.
+  intros.
+  specialize (H 0) as [L []].
   inversion H; subst.
-  assert (n = x0) by (eapply per_bot_var_inv; mauto 2).
-  subst.
+  inversion H0; subst.
+  reflexivity.
+Qed.
+
+Lemma per_subtyp_gvar_inv_left {P} (pred_P : PredicativeSig P) : forall {Δ x a b},
+    {{ SubT ⇑`! a x <: b ∈ per_subtyp pred_P Δ }} ->
+    exists a', b = d{{{ ⇑`! a' x }}}.
+Proof.
+  intros * H.
+  inversion_clear H.
+  specialize (H0 0) as [M []].
+  inversion H; subst.
+  inversion H0; subst.
+  eexists; reflexivity.
+Qed.
+
+Lemma per_subtyp_gvar_inv_right {P} (pred_P : PredicativeSig P) : forall {Δ x a b},
+    {{ SubT b <: ⇑`! a x ∈ per_subtyp pred_P Δ }} ->
+    exists a', b = d{{{ ⇑`! a' x }}}.
+Proof.
+  intros * H.
+  inversion_clear H.
+  specialize (H0 0) as [M []].
+  inversion H0; subst.
+  inversion H; subst.
   eexists; reflexivity.
 Qed.
