theories/Core/Semantic/Realizability.v
@@ -6,9 +6,9 @@ From McPTS.Core Require Import Base.
 From McPTS.Core.Semantic Require Export NbE PER.
 Import Domain_Notations.
 
-Lemma per_nat_then_per_top {P} : forall {n m : domain P},
-    {{ Dom n ≈ m ∈ per_nat }} ->
-    {{ Dom ⇓ ℕ n ≈ ⇓ ℕ m ∈ per_top }}.
+Lemma per_nat_then_per_top {P} : forall {Δ : gctx P} {n m},
+    {{ Dom n ≈ m ∈ per_nat Δ }} ->
+    {{ Dom ⇓ ℕ n ≈ ⇓ ℕ m ∈ per_top Δ }}.
 Proof with solve [destruct_conjs; eexists; repeat econstructor; eauto].
   induction 1; simpl in *; intros s;
     try specialize (IHper_nat s);
@@ -17,11 +17,11 @@ Qed.
 #[export]
 Hint Resolve per_nat_then_per_top : mcpts.
 
-Lemma realize_per_sort_elem_gen {P : PtsSig} {pred_P : PredicativeSig P} : forall {s a a' R},
-    {{ DF a ≈ a' ∈ per_sort_elem pred_P s ↘ R }} ->
-    {{ Dom a ≈ a' ∈ per_top_typ }}
-    /\ (forall {c c'}, {{ Dom c ≈ c' ∈ per_bot }} -> {{ Dom ⇑ a c ≈ ⇑ a' c' ∈ R }})
-    /\ (forall {b b'}, {{ Dom b ≈ b' ∈ R }} -> {{ Dom ⇓ a b ≈ ⇓ a' b' ∈ per_top }}).
+Lemma realize_per_sort_elem_gen {P : PtsSig} {pred_P : PredicativeSig P} : forall {Δ s a a' R},
+    {{ DF a ≈ a' ∈ per_sort_elem pred_P Δ s ↘ R }} ->
+    {{ Dom a ≈ a' ∈ per_top_typ Δ }}
+    /\ (forall {c c'}, {{ Dom c ≈ c' ∈ per_bot Δ }} -> {{ Dom ⇑ a c ≈ ⇑ a' c' ∈ R }})
+    /\ (forall {b b'}, {{ Dom b ≈ b' ∈ R }} -> {{ Dom ⇓ a b ≈ ⇓ a' b' ∈ per_top Δ }}).
 Proof with (solve [try (try (eexists; split); econstructor); mauto]).
   intros * Hsortelem. simpl in Hsortelem.
   induction Hsortelem using per_sort_elem_ind; repeat split; intros;
@@ -34,51 +34,51 @@ Proof with (solve [try (try (eexists; split); econstructor); mauto]).
     destruct_by_head (@per_sort P).
     specialize (H1 _ _ _ H).
     destruct_conjs.
-    intro s.
-    specialize (H0 s) as [? []]...
+    intro i.
+    specialize (H0 i) as [? []]...
   - destruct IHHsortelem as [? []].
-    intro s.
-    assert {{ Dom ⇑! a s ≈ ⇑! a' s ∈ in_rel }} by eauto using var_per_bot.
+    intro i.
+    assert {{ Dom ⇑! a i ≈ ⇑! a' i ∈ in_rel }} by eauto using var_per_bot.
     destruct_rel_mod_eval.
-    specialize (H9 (S s)) as [? []].
-    specialize (H2 s) as [? []]...
+    specialize (H9 (S i)) as [? []].
+    specialize (H2 i) as [? []]...
   - intros c0 c0' equiv_c0_c0'.
     destruct_conjs.
     destruct_rel_mod_eval.
     econstructor; try solve [econstructor; eauto].
-    enough ({{ Dom c ⇓ a c0 ≈ c' ⇓ a' c0' ∈ per_bot }}) by eauto.
-    intro s.
-    specialize (H3 s) as [? []].
-    specialize (H5 _ _ equiv_c0_c0' s) as [? []]...
+    enough ({{ Dom c ⇓ a c0 ≈ c' ⇓ a' c0' ∈ per_bot Δ }}) by eauto.
+    intro i.
+    specialize (H3 i) as [? []].
+    specialize (H5 _ _ equiv_c0_c0' i) as [? []]...
   - destruct_conjs.
-    intro s.
-    assert {{ Dom ⇑! a s ≈ ⇑! a' s ∈ in_rel }} by eauto using var_per_bot.
+    intro i.
+    assert {{ Dom ⇑! a i ≈ ⇑! a' i ∈ in_rel }} by eauto using var_per_bot.
     destruct_rel_mod_eval.
     destruct_rel_mod_app.
     match goal with
-    | _: {{ $| ^?f0 & ⇑! a s |↘ ^_ }},
-        _: {{ $| ^?f0' & ⇑! a' s |↘ ^_ }},
-          _: {{ ⟦ B ⟧ ρ ↦ ⇑! a s ↘ ^?b0 }},
-            _: {{ ⟦ B' ⟧ ρ' ↦ ⇑! a' s ↘ ^?b0' }} |- _ =>
+    | _: {{ ^?Δ ▶ $| ^?f0 & ⇑! a i |↘ ^_ }},
+        _: {{ ^?Δ ▶ $| ^?f0' & ⇑! a' i |↘ ^_ }},
+          _: {{ ^?Δ ▶ ⟦ B ⟧ ρ ↦ ⇑! a i ↘ ^?b0 }},
+            _: {{ ^?Δ ▶ ⟦ B' ⟧ ρ' ↦ ⇑! a' i ↘ ^?b0' }} |- _ =>
         rename f0 into f;
         rename f0' into f';
         rename b0 into b;
         rename b0' into b'
     end.
-    assert {{ Dom ⇓ b fa ≈ ⇓ b' f'a' ∈ per_top }} by eauto.
-    specialize (H2 s) as [? []].
-    specialize (H10 (S s)) as [? []].
-    specialize (H16 (S s)) as [? []]...
-  - intro s.
-    (on_all_hyp: fun H => destruct (H s) as [? []])...
-  - intro s.
+    assert {{ Dom ⇓ b fa ≈ ⇓ b' f'a' ∈ per_top Δ }} by eauto.
+    specialize (H2 i) as [? []].
+    specialize (H10 (S i)) as [? []].
+    specialize (H16 (S i)) as [? []]...
+  - intro i.
+    (on_all_hyp: fun H => destruct (H i) as [? []])...
+  - intro i.
     inversion_clear_by_head (@per_ne P).
-    (on_all_hyp: fun H => specialize (H s) as [? []])...
+    (on_all_hyp: fun H => specialize (H i) as [? []])...
 Qed.
 
-Corollary per_sort_then_per_top_typ {P : PtsSig} {pred_P : PredicativeSig P} : forall {s a a' R},
-    {{ DF a ≈ a' ∈ per_sort_elem pred_P s ↘ R }} ->
-    {{ Dom a ≈ a' ∈ per_top_typ }}.
+Corollary per_sort_then_per_top_typ {P : PtsSig} {pred_P : PredicativeSig P} : forall {Δ s a a' R},
+    {{ DF a ≈ a' ∈ per_sort_elem pred_P Δ s ↘ R }} ->
+    {{ Dom a ≈ a' ∈ per_top_typ Δ }}.
 Proof.
   intros * ?%realize_per_sort_elem_gen; firstorder.
 Qed.
@@ -86,9 +86,9 @@ Qed.
 #[export]
 Hint Resolve per_sort_then_per_top_typ : mcpts.
 
-Corollary per_bot_then_per_elem {P : PtsSig} {pred_P : PredicativeSig P} : forall {s a a' R c c'},
-    {{ DF a ≈ a' ∈ per_sort_elem pred_P s ↘ R }} ->
-    {{ Dom c ≈ c' ∈ per_bot }} -> {{ Dom ⇑ a c ≈ ⇑ a' c' ∈ R }}.
+Corollary per_bot_then_per_elem {P : PtsSig} {pred_P : PredicativeSig P} : forall {Δ s a a' R c c'},
+    {{ DF a ≈ a' ∈ per_sort_elem pred_P Δ s ↘ R }} ->
+    {{ Dom c ≈ c' ∈ per_bot Δ }} -> {{ Dom ⇑ a c ≈ ⇑ a' c' ∈ R }}.
 Proof.
   intros * ?%realize_per_sort_elem_gen; firstorder.
 Qed.
@@ -96,9 +96,9 @@ Qed.
 (** We cannot add [per_bot_then_per_elem] as a hint
     because we don't know what "R" is (i.e. the pattern becomes higher-order.)
     In fact, Coq complains it cannot add one if we try. *)
-Corollary per_elem_then_per_top {P : PtsSig} {pred_P : PredicativeSig P} : forall {s a a' R b b'},
-    {{ DF a ≈ a' ∈ per_sort_elem pred_P s ↘ R }} ->
-    {{ Dom b ≈ b' ∈ R }} -> {{ Dom ⇓ a b ≈ ⇓ a' b' ∈ per_top }}.
+Corollary per_elem_then_per_top {P : PtsSig} {pred_P : PredicativeSig P} : forall {Δ s a a' R b b'},
+    {{ DF a ≈ a' ∈ per_sort_elem pred_P Δ s ↘ R }} ->
+    {{ Dom b ≈ b' ∈ R }} -> {{ Dom ⇓ a b ≈ ⇓ a' b' ∈ per_top Δ }}.
 Proof.
   intros * ?%realize_per_sort_elem_gen; firstorder.
 Qed.
@@ -108,11 +108,11 @@ Hint Resolve per_elem_then_per_top : mcpts.
 
 
 (* Realizability for per_typ_elem *)
-Lemma realize_per_typ_elem_gen {P : PtsSig} {pred_P : PredicativeSig P} : forall {a a' R},
-    {{ DF a ≈ a' ∈ per_typ_elem pred_P ↘ R }} ->
-    {{ Dom a ≈ a' ∈ per_top_typ }}
-    /\ (forall {c c'}, {{ Dom c ≈ c' ∈ per_bot }} -> {{ Dom ⇑ a c ≈ ⇑ a' c' ∈ R }})
-    /\ (forall {b b'}, {{ Dom b ≈ b' ∈ R }} -> {{ Dom ⇓ a b ≈ ⇓ a' b' ∈ per_top }}).
+Lemma realize_per_typ_elem_gen {P : PtsSig} {pred_P : PredicativeSig P} : forall {Δ a a' R},
+    {{ DF a ≈ a' ∈ per_typ_elem pred_P Δ ↘ R }} ->
+    {{ Dom a ≈ a' ∈ per_top_typ Δ }}
+    /\ (forall {c c'}, {{ Dom c ≈ c' ∈ per_bot Δ }} -> {{ Dom ⇑ a c ≈ ⇑ a' c' ∈ R }})
+    /\ (forall {b b'}, {{ Dom b ≈ b' ∈ R }} -> {{ Dom ⇓ a b ≈ ⇓ a' b' ∈ per_top Δ }}).
 Proof with (solve [try (try (eexists; split); econstructor); mauto]).
   intros * Htypelem. simpl in Htypelem.
   induction Htypelem.
@@ -120,25 +120,23 @@ Proof with (solve [try (try (eexists; split); econstructor); mauto]).
     + econstructor; mauto.
     + intros.
       apply_relation_equivalence.
-      exists per_ne.
+      exists (per_ne Δ).
       per_sort_elem_econstructor; mauto.
       reflexivity.
     + intros.
       apply_relation_equivalence.
       unfold per_sort in H0.
       destruct_conjs.
-      assert ({{ Dom b ≈ b' ∈ (@per_top_typ P) }}) by mauto.
-      simpl in H1.
+      assert ({{ Dom b ≈ b' ∈ per_top_typ Δ }}) by mauto.
       intros n.
-      assert (exists C : nf P, {{ Rtyp b in n ↘ C }} /\ {{ Rtyp b' in n ↘ C }}) by mauto.
-      destruct_conjs.
+      specialize (H1 n) as [M []].
       econstructor; mauto.
   - eapply realize_per_sort_elem_gen; mauto.
 Qed.
 
-Corollary per_typ_elem_then_per_top_typ {P : PtsSig} {pred_P : PredicativeSig P} : forall {a a' R},
-    {{ DF a ≈ a' ∈ per_typ_elem pred_P ↘ R }} ->
-    {{ Dom a ≈ a' ∈ per_top_typ }}.
+Corollary per_typ_elem_then_per_top_typ {P : PtsSig} {pred_P : PredicativeSig P} : forall {Δ a a' R},
+    {{ DF a ≈ a' ∈ per_typ_elem pred_P Δ ↘ R }} ->
+    {{ Dom a ≈ a' ∈ per_top_typ Δ }}.
 Proof.
   intros * ?%realize_per_typ_elem_gen; firstorder.
 Qed.
@@ -146,9 +144,9 @@ Qed.
 #[export]
 Hint Resolve per_typ_elem_then_per_top_typ : mcpts.
 
-Corollary per_bot_then_per_typ_elem {P : PtsSig} {pred_P : PredicativeSig P} : forall {a a' R c c'},
-    {{ DF a ≈ a' ∈ per_typ_elem pred_P ↘ R }} ->
-    {{ Dom c ≈ c' ∈ per_bot }} -> {{ Dom ⇑ a c ≈ ⇑ a' c' ∈ R }}.
+Corollary per_bot_then_per_typ_elem {P : PtsSig} {pred_P : PredicativeSig P} : forall {Δ a a' R c c'},
+    {{ DF a ≈ a' ∈ per_typ_elem pred_P Δ ↘ R }} ->
+    {{ Dom c ≈ c' ∈ per_bot Δ }} -> {{ Dom ⇑ a c ≈ ⇑ a' c' ∈ R }}.
 Proof.
   intros * ?%realize_per_typ_elem_gen; firstorder.
 Qed.
@@ -156,9 +154,9 @@ Qed.
 (** We cannot add [per_bot_then_per_elem] as a hint
     because we don't know what "R" is (i.e. the pattern becomes higher-order.)
     In fact, Coq complains it cannot add one if we try. *)
-Corollary per_typ_elem_then_per_top {P : PtsSig} {pred_P : PredicativeSig P} : forall {a a' R b b'},
-    {{ DF a ≈ a' ∈ per_typ_elem pred_P ↘ R }} ->
-    {{ Dom b ≈ b' ∈ R }} -> {{ Dom ⇓ a b ≈ ⇓ a' b' ∈ per_top }}.
+Corollary per_typ_elem_then_per_top {P : PtsSig} {pred_P : PredicativeSig P} : forall {Δ a a' R b b'},
+    {{ DF a ≈ a' ∈ per_typ_elem pred_P Δ ↘ R }} ->
+    {{ Dom b ≈ b' ∈ R }} -> {{ Dom ⇓ a b ≈ ⇓ a' b' ∈ per_top Δ }}.
 Proof.
   intros * ?%realize_per_typ_elem_gen; firstorder.
 Qed.
@@ -166,9 +164,9 @@ Qed.
 #[export]
 Hint Resolve per_typ_elem_then_per_top : mcpts.
 
-Lemma per_ctx_then_per_env_initial_env {P : PtsSig} {pred_P : PredicativeSig P} : forall {Γ Γ' env_rel},
-    {{ EF Γ ≈ Γ' ∈ per_ctx_env pred_P ↘ env_rel }} ->
-    exists ρ ρ', initial_env Γ ρ /\ initial_env Γ' ρ' /\ {{ Dom ρ ≈ ρ' ∈ env_rel }}.
+Lemma per_ctx_then_per_env_initial_env {P : PtsSig} {pred_P : PredicativeSig P} : forall {Δ Γ Γ' env_rel},
+    {{ EF Γ ≈ Γ' ∈ per_ctx_env pred_P Δ ↘ env_rel }} ->
+    exists ρ ρ', initial_env Δ Γ ρ /\ initial_env Δ Γ' ρ' /\ {{ Dom ρ ≈ ρ' ∈ env_rel }}.
 Proof.
   induction 1.
   - do 2 eexists; intuition.
@@ -182,10 +180,18 @@ Proof.
     eexists; eauto.
 Qed.
 
-Lemma var_per_elem {P : PtsSig} {pred_P : PredicativeSig P} : forall {a b s R} n,
-    {{ DF a ≈ b ∈ per_sort_elem pred_P s ↘ R }} ->
+Lemma var_per_elem {P : PtsSig} {pred_P : PredicativeSig P} : forall {Δ a b s R} n,
+    {{ DF a ≈ b ∈ per_sort_elem pred_P Δ s ↘ R }} ->
     {{ Dom ⇑! a n ≈ ⇑! b n ∈ R }}.
 Proof.
   intros.
   eapply per_bot_then_per_elem; mauto.
+Qed.
+
+Lemma var_per_typ_elem {P : PtsSig} {pred_P : PredicativeSig P} : forall {Δ a b R} n,
+    {{ DF a ≈ b ∈ per_typ_elem pred_P Δ ↘ R }} ->
+    {{ Dom ⇑! a n ≈ ⇑! b n ∈ R }}.
+Proof.
+  intros.
+  eapply per_bot_then_per_typ_elem; mauto.
 Qed.
